Switched from MEquiv to table_wf. Finished derived specs for partial_table. Commented out fold in concurrent.

concurrent/hashtable.v
@@ -2,29 +2,23 @@ From stdpp Require Export set.
 From iris.proofmode Require Import tactics.
 From iris.algebra Require Import auth.
 From iris.base_logic Require Import big_op.
+From iris.base_logic.lib Require Import fractional.
 From iris.program_logic Require Import hoare.
 From iris.heap_lang Require Export proofmode lang lifting notation.
-From iris.heap_lang.lib Require Import lock.
+From iris.heap_lang.lib Require Export lock.
 From iris_programs.iterators Require Export hashtable_model.
-From iris_programs.iterators Require Import hashtable_fin_map hashtable_invariants util.
-From iris_programs Require Import forloop for_test.
-From iris_programs.concurrent Require Export array.
+From iris_programs.iterators Require Import util modulo.
+From iris_programs Require Import forloop array hashtable_buckets.
 
-
-Class tableG Σ := {table_inG :> inG Σ (authR (optionUR (exclR (leibnizC BucketData))))}.
+(*Class tableG Σ := {table_inG :> inG Σ (authR (optionUR (exclR (leibnizC bucket_data))))}.*)
 
 Section hashtable.
 
-  Local Definition some_excl (b: BucketData) :=
-    Some (Excl b : exclR _): optionUR (exclR (leibnizC BucketData)).
-  
-  Context Σ Key Hash `{Hashable Σ Key Hash} `{!Array Σ} `{!tableG Σ}.
-  Context Map `{FinMap Key Map}.
+ (* Local Definition some_excl (b: bucket_data) :=
+    Some (Excl b : exclR _): optionUR (exclR (leibnizC bucket_data)).
+  *)
+  Context Σ Key Hash map `{FinMap Key map , heapG Σ, !Hashable Σ Key Hash, !Array Σ(*, !tableG Σ*)}.
   Variable lck : lock Σ.
-  Variable modulo: val.
-  Hypothesis modulo_spec:
-    forall (m n : Z), WP modulo (#m, #n) {{v, ⌜v = #(m `mod` n)⌝}}%I.
-
 
   Definition create_table : val :=
     λ: "n", let: "arr" := make_array ("n",#()) in
@@ -112,36 +106,11 @@ Section hashtable.
           "a") #0 "a".
   
 
-  Implicit Type M : Map (list val).
-  Arguments content {_ _ _ _ _ _ _ _ _} _ _.
-  Arguments no_garbage {_ _ _ _ _ _ _} _.
-  Arguments have_keys {_ _ _ _ _ _} _.
-
-  (*Definition hashtable_inv P M arr refs locks :=
-    (array arr (zip_with PairV (LitV ∘ LitLoc <$> refs) locks) ∗
-     table_inv P M)%I.
-  
-  Definition is_table N P t : iProp Σ :=
-    (∃ arr refs locks M data,
-        ⌜t = (arr, #(length data))%V⌝ ∗
-        ⌜content M data⌝ ∗
-        ⌜no_garbage data⌝ ∗
-        ⌜have_keys data⌝ ∗
-        ⌜length data > 0⌝ ∗
-        ⌜length refs = length data⌝ ∗
-        ⌜length locks = length data⌝ ∗
-        ([∗ list] lrb ∈ zip (zip locks refs) data,
-          let '((l, r), b) := lrb in
-          ∃ γ, is_lock lck N γ l (r ↦  bucket b)) ∗
-        inv N (hashtable_inv P M arr refs locks))%I.
-                
-  Instance is_locks_persistent N lrb :
-    PersistentP
-      (let '(l, r, b) := lrb in
-       (∃ γ : name Σ lck, is_lock lck N γ l (r ↦ bucket b))%I).
-  Proof. destruct lrb as [[? ?] ?]. typeclasses eauto. Qed.
-*)
-
+  Implicit Type m : map (list val).
+  Local Arguments content {_ _ _ _ _ _ _ _} _ _.
+  Local Arguments no_garbage {_ _ _ _ _ _} _.
+  Local Arguments have_keys {_ _ _ _ _ _} _.
+(*
   Definition is_table N P t : iProp Σ :=
     (∃ arr refs locks,
         ⌜t = (arr, #(length refs))%V⌝ ∗
@@ -163,9 +132,30 @@ Section hashtable.
   Proof. destruct lr as [? ?]. typeclasses eauto. Qed.
   
   Global Instance is_table_persistent N P t : PersistentP (is_table N P t).
-  Proof. typeclasses eauto. Qed.
+  Proof. typeclasses eauto. Qed.*)
+
+  Definition is_table N P t :=
+   (∃ arr refs locks, 
+      ⌜t = (arr, #(length refs))%V⌝ ∗
+      ⌜length refs > 0⌝ ∗
+      ⌜length refs = length locks⌝ ∗
+      ([∗ list] i ↦ lr ∈ zip locks refs,
+        let '(l, r) := lr in
+        ∃ lname, is_lock lck (N.@(S i)) lname l (r ↦{1/2} -)) ∗
+      inv (N.@0)
+       (array arr (zip_with PairV (LitV ∘ LitLoc <$> refs) locks) ∗
+        ∃ m data,
+          ⌜table_wf m⌝ ∗
+          ⌜content m data⌝ ∗
+          ⌜no_garbage data⌝ ∗
+          ⌜have_keys data⌝ ∗
+          ⌜length data = length refs⌝ ∗
+          P m ∗ 
+          [∗ list] rb ∈ zip refs data,
+           let '(r, b) := rb in
+           r ↦{1/2} bucket b))%I.
   
-  Definition is_table_alt N P t :=
+ (* Definition is_table N P t :=
    (∃ arr refs locks γs, 
       ⌜t = (arr, #(length refs))%V⌝ ∗
       ⌜length refs > 0⌝ ∗
@@ -176,16 +166,17 @@ Section hashtable.
         ∃ lname, is_lock lck (N.@(S i)) lname l (∃ b', own γ (● some_excl b'))) ∗
       inv (N.@0)
        (array arr (zip_with PairV (LitV ∘ LitLoc <$> refs) locks) ∗
-        ∃ M data,
-          ⌜content M data⌝ ∗
+        ∃ m data,
+          ⌜table_wf m⌝ ∗
+          ⌜content m data⌝ ∗
           ⌜no_garbage data⌝ ∗
           ⌜have_keys data⌝ ∗
           ⌜length data = length refs⌝ ∗
-          P M ∗ 
+          P m ∗ 
           [∗ list] rbγ ∈ zip (zip refs data) γs,
            let '(r, b, γ) := rbγ in
-           r ↦ bucket b ∗ own γ (◯ some_excl b)))%I.
-
+           r ↦ bucket b ∗ own γ (◯ some_excl b)))%I.*)
+(*
   Lemma table_own_eq γ b b' :
     ((own γ (● some_excl b) ∗ own γ (◯ some_excl b')) → ⌜b' = b⌝)%I.
   Proof.
@@ -206,39 +197,22 @@ Section hashtable.
   Proof.
     iIntros "Ha Hp". iApply own_op.
     iApply own_update. apply auth_update.
-    apply (option_local_update (A:=exclR (leibnizC BucketData))).
+    apply (option_local_update (A:=exclR (leibnizC bucket_data))).
     eapply exclusive_local_update. done.
     iApply own_op.
     iFrame. Unshelve. apply _.
   Qed.    
-    
-  Global Instance is_table_alt_persistent N P t : PersistentP (is_table_alt N P t).
+*)
+ Instance is_locks_persistent N `(lr : (val * B)) P:
+    PersistentP
+      (let (l, r) := lr in
+          ∃ γ, is_lock lck (N.@(S i)) γ l (P l r))%I.
+  Proof. destruct lr as [? ?]. typeclasses eauto. Qed.
+  
+  Global Instance is_table_persistent N P t : PersistentP (is_table N P t).
   Proof. typeclasses eauto. Qed.
-
   
-  (*Definition table_in_state N M (data : list BucketData) arr n :=
-    ( ⌜length data > 0⌝ ∗
-      ⌜content M data⌝ ∗
-      ⌜no_garbage data⌝ ∗
-      ⌜have_keys data⌝ ∗
-      ⌜n = length data⌝ ∗
-      ∃ refs locks,
-        ⌜length data = length refs⌝ ∗
-        ⌜length data = length locks⌝ ∗
-        array arr (zip_with PairV (LitV ∘ LitLoc <$> refs) locks) ∗
-        [∗ list] lrb ∈ zip (zip locks refs) data,
-          let '((l, r), b) := lrb in
-          ∃ γ, is_lock lck N γ l (r ↦  bucket b)                           
-    )%I.
-  
-  Definition is_table N P t : iProp Σ :=
-    (∃ arr (n : nat), ⌜t = (arr, #n)%V⌝ ∗
-          inv N (∃ M data, table_in_state N M data arr n ∗ table_inv P M))%I.*)
-
-
-  Ltac rename_last H' := match goal with [H : _ |- _] => rename H into H' end ; move H' at top.
-  
-  Lemma create_table_spec N P n : n > 0 -> WP create_table #n {{t, is_table N P t}}%I.
+(*  Lemma create_table_spec N P n : n > 0 -> WP create_table #n {{t, is_table N P t}}%I.
   Proof.
     intro Hn.
     wp_lam. wp_bind (make_array _). iApply wp_wand.
@@ -284,9 +258,73 @@ Section hashtable.
       repeat (iSplit ; first eauto ).
       iExact "HInv".
       iNext. by rewrite -minus_n_n /= app_nil_r.
-  Qed.
+  Qed.*)
 
-  Lemma create_table_spec2 N P n : n > 0 -> {{{P ∅}}} create_table #n {{{t, RET t ; is_table_alt N P t}}}.
+Lemma create_table_spec N P n : n > 0 -> {{{P ∅}}} create_table #n {{{t, RET t ; is_table N P t}}}.
+  Proof.
+    iIntros (Hn Φ) "HP HΦ".
+    wp_lam. wp_bind (make_array _). iApply wp_wand.
+    iApply (make_array_spec _ #()). iIntros (arr) "Harr". wp_lam.   
+    
+    wp_for (fun i' : Z =>
+              ∃ locks refs (i : nat),
+                ⌜i' = i⌝ ∗
+                ⌜i = length refs⌝ ∗
+                ⌜i = length locks⌝ ∗
+                array arr (zip_with PairV (LitV ∘ LitLoc <$> refs) locks ++ replicate (n - i) #()) ∗
+                [∗ list] i ↦ lr ∈ zip locks refs,
+                  (lr.2) ↦{1/2} NONEV ∗
+                  ∃ lname, is_lock lck (N.@(S i)) lname (lr.1)
+                               ((lr.2) ↦{1/2}-))%I with "[Harr]". 
+    - iExists [], [], 0. rewrite big_sepL_nil -minus_n_O /=. by iFrame.
+    - iIntros (i') "% HInv".
+      iDestruct "HInv" as (locks refs i) "[% [% [% [Harr Hlr]]]]".
+      simplify_eq. wp_alloc r as "Hr".
+      iDestruct (fractional_half_1 with "Hr") as "[Hr1 Hr2]". 
+      wp_apply (newlock_spec _ _ (N.@(S (length refs))) with "[Hr1]") ; last first.
+      iIntros (lk lname) "Hlk".
+      wp_apply (array_store_spec _ _ (#r, lk) with "[Harr]") ; [|done|].
+      rewrite app_length replicate_length zip_with_length fmap_length. lia.
+      iIntros "Harr". iExists (locks ++ [lk]), (refs ++ [r]), (S (length refs)).
+      do 2 rewrite app_length. simpl.
+      do 3 (iSplit ; first (iPureIntro ; lia)).
+      iSplitL "Harr". rewrite fmap_app zip_with_app ; last by rewrite fmap_length.
+      rewrite {1}(plus_n_O (length refs))
+        -{1}(fmap_length (LitV ∘ LitLoc) refs)
+        -(zip_with_length_l_eq PairV (LitV ∘ LitLoc <$> refs) locks) ; last by rewrite fmap_length.
+      rewrite insert_app_r.
+      rewrite (_:n = S (pred n)) ; last lia.
+      rewrite -minus_Sn_m ; last lia.
+      rewrite replicate_S /= cons_middle app_assoc. iFrame.
+      rewrite zip_with_app ; last done.
+      iApply big_sepL_app. iFrame.
+      rewrite -plus_n_O zip_with_length_r_eq /= //. eauto.
+      eauto.
+    - iIntros "HInv". iDestruct "HInv" as (locks refs ?) "[% [% [% [Harr Hlrs]]]]".
+      iDestruct (big_sepL_sepL with "Hlrs") as "[Hparts #Hlks]".
+      simplify_eq. iMod (inv_alloc (N.@0) _  with "[-HΦ]") as "#HInv" ; last first.
+      wp_lam. iApply "HΦ". iExists arr, refs, locks.
+      repeat (iSplit ; first eauto).
+      repeat rewrite big_sepL_zip_with.
+      iApply (big_sepL_mono with "Hlks").
+      iIntros (i lk ?) "Hlks". iIntros (r ?).
+      iDestruct ("Hlks" $! r with "[]") as "$". done.
+      iExact "HInv".
+      iNext. rewrite -minus_n_n /= app_nil_r.
+      iFrame. iExists ∅, (replicate (length refs) []).
+      repeat (iSplit ; first eauto using table_wf_empty, content_empty, no_garbage_empty, have_keys_empty, replicate_length).
+      iFrame.
+      rewrite {2}(zip_with_flip _ refs).
+      repeat rewrite big_sepL_zip_with.
+      iApply (big_sepL_mono with "Hparts").
+      iIntros (i r ?) "Hlrs". iIntros (b Hb).
+      apply lookup_replicate in Hb. destruct Hb as [-> ?].
+      assert (is_Some (locks !! i)) as [lk ?].
+      { apply lookup_lt_is_Some. by rewrite -(_:length refs = length locks). }
+      iDestruct ("Hlrs" $! lk with "[]") as "Hlr" ; done.
+  Qed.
+  
+  (*Lemma create_table_spec N P n : n > 0 -> {{{P ∅}}} create_table #n {{{t, RET t ; is_table N P t}}}.
   Proof.
     iIntros (Hn Φ) "HP HΦ".
     wp_lam. wp_bind (make_array _). iApply wp_wand.
@@ -349,7 +387,7 @@ Section hashtable.
       iExact "HInv".
       iNext. rewrite -minus_n_n /= app_nil_r.
       iFrame. iExists ∅, (replicate (length refs) []).
-      repeat (iSplit ; first eauto using content_empty, no_garbage_empty, have_keys_empty, replicate_length).
+      repeat (iSplit ; first eauto using table_wf_empty, content_empty, no_garbage_empty, have_keys_empty, replicate_length).
       iFrame. iCombine "Hparts Hrs" as "Hlrs".
       rewrite {2}(zip_with_flip _ refs).
       repeat rewrite big_sepL_zip_with.
@@ -361,7 +399,7 @@ Section hashtable.
       iDestruct ("Hlrs" $! lk with "[]") as "Hlr" ; first done.
       iDestruct ("Hlr" $! γ with "[]") as "[? ?]" ; first done.
       iFrame.
-  Qed.
+  Qed.*)
 
   Lemma index_spec (k : val) k' (n : nat) :
     as_key k = Some k' ->
@@ -380,7 +418,7 @@ Section hashtable.
     by rewrite Z2Nat_inj_mod.
   Qed.
   
-  Lemma table_insert_spec N P k k' x t:
+ (* Lemma table_insert_spec N P k k' x t:
     as_key k' = Some k ->
     {{{P k x ∗ is_table N P t}}} table_insert t k' x {{{RET #(); True}}}.
   Proof.
@@ -409,16 +447,16 @@ Section hashtable.
     iFrame "Hlock Hlocked". iExists ((k', x)::b). iFrame. iApply big_sepL_cons. iFrame.
     iExists k. eauto.
     iIntros "_". by iApply "HΦ".
-  Qed.
+  Qed.*)
 
-    Lemma table_insert_spec2 N P Q k k' x t:
+  Lemma table_insert_spec N P Q k k' x t:
     as_key k' = Some k ->
-    {{{is_table_alt N P t ∗ ∀ M, P M ={⊤∖↑N}=∗ P (insert_val M k x) ∗ Q }}}
+    {{{is_table N P t ∗ ∀ m, P m ={⊤∖↑N}=∗ P (insert_val m k x) ∗ Q }}}
       table_insert t k' x {{{RET #(); Q}}}.
   Proof.
     iIntros (Hkey Φ) "[#HTable HPins] HΦ".
-    iDestruct "HTable" as (arr refs locks γs) "[% [% [% [% [Hlocks HInv]]]]]".
-    rename_last Hrefs_γs. rename_last Hrefs_locks.
+    iDestruct "HTable" as (arr refs locks) "[% [% [% [Hlocks HInv]]]]".
+    rename_last Hrefs_locks.
     simplify_eq.
     do 3 wp_lam. wp_proj. wp_lam. wp_proj. wp_lam. wp_bind (index _ _).
     iApply wp_wand. iApply (index_spec _ _ _ Hkey).
@@ -429,49 +467,47 @@ Section hashtable.
       apply mod_bound_pos. lia. done. }
     assert (is_Some (refs !! (Hash k `mod` length refs))) as [r Hr].
     { apply lookup_lt_is_Some. apply mod_bound_pos. lia. done. }
-    assert (is_Some (γs !! (Hash k `mod` length refs))) as [γ Hγ].
-    { apply lookup_lt_is_Some. rewrite -Hrefs_γs.
-      apply mod_bound_pos. lia. done. }
     wp_apply (array_load_spec _ _ (#r, lk) (Hash k `mod` length refs) with "Harr").
     by rewrite lookup_zip_with list_lookup_fmap Hlk Hr. 
     iIntros "Harr". iMod ("HClose" with "[Harr Hrest]") as "_"; first (iNext; iFrame).
     iModIntro. wp_lam. wp_proj. wp_lam. wp_proj. wp_lam.
-    iDestruct (big_sepL_lookup _ _ _ (lk, γ)  with "Hlocks") as (lname) "Hlock".
-    by erewrite lookup_zip_with, Hlk, Hγ.
+    iDestruct (big_sepL_lookup _ _ _ (lk, r)  with "Hlocks") as (lname) "Hlock".
+    by erewrite lookup_zip_with, Hlk, Hr.
     wp_apply (acquire_spec with "Hlock").
-    iIntros "[Hlocked Hauth]". iDestruct "Hauth" as (b) "Hauth".
+    iIntros "[Hlocked Hr1]". iDestruct "Hr1" as (?) "Hr1".
     wp_lam. wp_bind (! _)%E.
     iInv (N.@0) as "[Harr Hrest]" "HClose".
-    iDestruct "Hrest" as (M data) "[>% [>% [>% [>% [HP Hrbγs]]]]]".
+    iDestruct "Hrest" as (m data) "[>% [>% [>% [>% [>% [HP Hrbs]]]]]]".
     rename_last Hdata_refs.
-    assert (is_Some (data !! (Hash k `mod` length refs))) as [b' Hb'].
+    assert (is_Some (data !! (Hash k `mod` length refs))) as [b Hb].
     { apply lookup_lt_is_Some. rewrite Hdata_refs.
       apply mod_bound_pos. lia. done. }
-    iDestruct (big_sepL_lookup_acc _ _ _ (r, b', γ) with "Hrbγs") as "[[HrPtr >Hpart] Hrbγs]".
-    by erewrite lookup_zip_with, lookup_zip_with, Hr, Hb', Hγ.
-    iDestruct (table_own_eq with "[$Hpart $Hauth]") as "%". simplify_eq.
+    iDestruct (big_sepL_lookup_acc _ _ _ (r, b) with "Hrbs") as "[>Hr2 Hrbs]".
+    by erewrite lookup_zip_with, Hr, Hb.
+    iDestruct (mapsto_agree with "Hr1 Hr2") as "%". simplify_eq.
     wp_load.
-    iMod ("HClose" with "[Harr HP HrPtr Hpart Hrbγs]") as "_".
-    iDestruct ("Hrbγs" with "[$HrPtr $Hpart]") as "?". iFrame. iExists M, data. iFrame. eauto.
-    iModIntro. clear dependent M data. wp_bind (_ <- _)%E.
+    iMod ("HClose" with "[Harr HP Hr2 Hrbs]") as "_".
+    iDestruct ("Hrbs" with "Hr2") as "?". iFrame. iExists m, data. iFrame. eauto.
+    iModIntro. clear dependent m data. wp_bind (_ <- _)%E.
     iInv (N.@0) as "[Harr Hrest]" "HClose".
-    iDestruct "Hrest" as (M data) "[>% [>% [>% [>% [HP Hrbγs]]]]]".
+    iDestruct "Hrest" as (m data) "[>% [>% [>% [>% [>% [HP Hrbs]]]]]]".
     rename_last Hdata_refs.
     assert (is_Some (data !! (Hash k `mod` length refs))) as [b' Hb'].
     { apply lookup_lt_is_Some. rewrite Hdata_refs.
       apply mod_bound_pos. lia. done. }
-    rewrite -{1}(take_drop_middle _ _ _ Hb') -{6}(take_drop_middle _ _ _ Hr) -{3}(take_drop_middle _ _ _ Hγ).
+    rewrite -{1}(take_drop_middle _ _ _ Hb') -{7}(take_drop_middle _ _ _ Hr).
     repeat rewrite zip_with_app. repeat rewrite zip_with_cons.
-    iDestruct (big_sepL_app with "Hrbγs") as "[Htake Hdrop]".
-    iDestruct (big_sepL_cons with "Hdrop") as "[[HrPtr >Hpart] Hdrop]".
-    iDestruct (table_own_eq with "[$Hpart $Hauth]") as "%". simplify_eq.
-    wp_store.
-    iDestruct (table_own_update _ _ ((k', x)::b) with "Hauth Hpart") as ">[Hauth Hpart]".
+    iDestruct (big_sepL_app with "Hrbs") as "[Htake Hdrop]".
+    iDestruct (big_sepL_cons with "Hdrop") as "[>Hr2 Hdrop]".
+    iDestruct (mapsto_agree with "Hr1 Hr2") as "%". rename_last HbEq. rewrite HbEq.
+    iDestruct (fractional_half_2 with "Hr1 Hr2") as "Hr". apply _. wp_store.
     iDestruct ("HPins" with "HP") as "HPins".
-    iDestruct (fupd_mask_mono _ (⊤ ∖ ↑N.@0) with "HPins") as ">[HP HQ]". solve_ndisj. 
-    iMod ("HClose" with "[-Hauth HΦ Hlocked HQ]") as "_".
+    iDestruct (fupd_mask_mono _ (⊤ ∖ ↑N.@0) with "HPins") as ">[HP HQ]". solve_ndisj.
+    iDestruct "Hr" as "[Hr1 Hr2]".
+    iMod ("HClose" with "[-Hr1 HΦ Hlocked HQ]") as "_".
     {
-      iFrame. iExists (insert_val M k x), (insert_data _ _ data k (k', x)). iFrame. iNext.
+      iFrame. iExists (insert_val m k x), (insert_data _ _ data k (k', x)). iFrame. iNext.
+      iSplit. iPureIntro. by apply table_wf_insert_val.
       iSplit. iPureIntro. eapply content_insert ; try first [done | apply _ | lia].
       iSplit. iPureIntro. by apply no_garbage_insert.
       iSplit. iPureIntro. by apply have_keys_insert.
@@ -479,30 +515,24 @@ Section hashtable.
       erewrite <-(take_drop_middle (insert_data _ _ _ _ _)).
       rewrite /insert_data take_insert ; last reflexivity.
       rewrite drop_insert ; last lia.
-      rewrite -{13}(take_drop_middle _ _ _ Hr) -{6}(take_drop_middle _ _ _ Hγ).
+      rewrite -{12}(take_drop_middle _ _ _ Hr).
       repeat rewrite zip_with_app. repeat rewrite zip_with_cons.
       rewrite big_sepL_app big_sepL_cons Hdata_refs.
-      iFrame.
-      by rewrite zip_with_length_l_eq take_length take_length ;
-        try rewrite Hdata_refs ;
-        try rewrite -Hrefs_γs.
-      do 2 rewrite take_length. rewrite Hdata_refs //.
+      iFrame. rewrite /bucket -/(bucket ((k', x) :: b')). iApply "Hr2".
+      rewrite take_length take_length Hdata_refs //.
       rewrite /insert_data /lookup_data Hdata_refs.
       rewrite Hb' /=. apply list_lookup_insert.
       rewrite Hdata_refs.
       apply mod_bound_pos ; [lia|done].
     }
     iModIntro. wp_lam.
-    wp_apply (release_spec with "[Hlocked Hauth]"). iFrame "Hlock Hlocked".
+    wp_apply (release_spec with "[Hlocked Hr1]"). iFrame "Hlock Hlocked".
     eauto. iIntros. iApply ("HΦ" with "HQ").
    
-    rewrite zip_with_length_l_eq take_length take_length ;
-      try rewrite Hdata_refs //;
-      try rewrite -Hrefs_γs //.
-    do 2 rewrite take_length. rewrite Hdata_refs //.
+    rewrite 2!take_length Hdata_refs //.
   Qed.
 
-  Lemma table_remove_spec N P k k' t:
+(*  Lemma table_remove_spec N P k k' t:
     as_key k' = Some k ->
     {{{is_table N P t}}}
       table_remove t k'
@@ -611,19 +641,183 @@ Section hashtable.
 
   Lemma fmap_head {A B} (f : A -> B) (l: list A) :
     head (f <$> l) = f <$> head l.
-  Proof. by case l. Qed.
-    
-  Lemma table_remove_spec2 N P Q Q' k k' t:
+  Proof. by case l. Qed.*)
+
+  Lemma table_remove_spec N P Q Q' k k' t:
     as_key k' = Some k ->
-    {{{is_table_alt N P t ∗
-       (∀ M,
-         ⌜head (lookup_all M k) = None⌝ -∗ P M -∗ P M ∗ Q') ∗
-       ∀ M x,
-         ⌜head (lookup_all M k) = Some x⌝ -∗ P M -∗ P (remove_val M k) ∗ Q k x}}}
+    {{{is_table N P t ∗
+       (∀ m,
+         ⌜m !! k = None⌝ -∗ P m ={⊤∖↑N}=∗ P m ∗ Q') ∧
+       ∀ m x xs,
+         ⌜m !! k = Some (x :: xs)⌝ -∗ P m ={⊤∖↑N}=∗ P (remove_val m k) ∗ Q k x}}}
       table_remove t k'
       {{{v x, RET v; ⌜v = NONEV⌝ ∗ Q' ∨ (⌜v = SOMEV x⌝ ∗ Q k x)}}}.
   Proof.
-    iIntros (HKey Φ) "[HTable [HQ' HQ]] HΦ".
+    iIntros (HKey Φ) "[HTable HQ] HΦ".
+    iDestruct "HTable" as (arr refs locks) "[% [% [% [#Hlocks #HInv]]]]".
+    rename_last Hrefs_locks. simplify_eq.
+    do 2 wp_lam. wp_proj. wp_lam. wp_proj. wp_lam.
+    wp_bind (index _ _). iApply wp_wand. iApply index_spec. exact HKey.
+    iIntros (?) "%". simplify_eq.
+    wp_bind (array_load _).
+    iInv (N.@0) as "[Harr Hrest]" "HClose".
+    assert (is_Some (locks !! (Hash k `mod` length refs))) as [lk Hlk].
+    { apply lookup_lt_is_Some. rewrite -Hrefs_locks.
+      apply mod_bound_pos. lia. done. }
+    assert (is_Some (refs !! (Hash k `mod` length refs))) as [r Hr].
+    { apply lookup_lt_is_Some. apply mod_bound_pos. lia. done. }
+    wp_apply (array_load_spec _ _ (#r, lk) (Hash k `mod` length refs) with "Harr").
+    by rewrite lookup_zip_with list_lookup_fmap Hlk Hr.
+    iIntros "Harr". iMod ("HClose" with "[$Harr $Hrest]") as "_".
+    iModIntro. wp_lam. wp_proj. wp_lam. wp_proj. wp_lam.
+    iDestruct (big_sepL_lookup _ _ _ (lk, r) with "Hlocks") as (lname) "Hlock".
+    erewrite lookup_zip_with, Hlk, Hr. reflexivity.
+    wp_apply (acquire_spec with "Hlock").
+    iIntros "[Hlocked Hr1]".
+    iDestruct "Hr1" as (?) "Hr1". wp_lam. wp_bind (! _)%E.
+    iInv (N.@0) as "[Harr Hrest]" "HClose".
+    iDestruct "Hrest" as (m data) "[>% [>% [>% [>% [>% [HP Hrbs]]]]]]".
+    rename_last Hdata_refs. rename_last HHKeys. rename_last HNG. rename_last Hcontent. rename_last Hwf.
+    assert (is_Some (data !! (Hash k `mod` length refs))) as [b Hb].
+    { apply lookup_lt_is_Some. rewrite (_:length data = length refs) ; last done.
+      apply mod_bound_pos. lia. done. }
+    iDestruct (big_sepL_lookup_acc _ _ _ (r, b) with "Hrbs") as "[>Hr2 Hrbs]".
+    by erewrite lookup_zip_with, Hr, Hb.
+    iDestruct (mapsto_agree with "Hr1 Hr2") as "%". simplify_eq.
+    wp_load.
+
+    iAssert (WP (rec: "go" "b"
+                 := match: "b" with
+                      InjL <> => InjL #()
+                    | InjR "kxb" =>
+                      let: "k'" := Fst (Fst "kxb") in
+                      let: "x" := Snd (Fst "kxb") in
+                      let: "b" := Snd "kxb" in
+                      if: (equalf k') "k'" then InjR ("x", "b")
+                      else match: "go" "b" with
+                             InjL <> => InjL #()
+                           | InjR "p" =>
+                             InjR (Fst "p", InjR ("k'", "x", Snd "p"))
+                           end
+                    end) (bucket b)
+                {{v,  ⌜(v = NONEV /\ bucket_filter _ _ Hash k b = []) ∨
+                       (∃ k'' x b' b'',
+                           bucket_filter _ _ Hash k b = (k'', x)::b'' /\
+                           v = SOMEV (x, bucket b') /\
+                           b' = bucket_remove _ _ Hash k b)⌝}})%I as "Hloop".
+    { assert (Hsuff: b = [] ++ b) by done.
+      assert (Hpref: [] = bucket_filter _ _ Hash k []) by done.
+      revert Hsuff Hpref. generalize b at 2 3 4 5 6. generalize ([] : bucket_data) at 1 3.
+      intros b'' b' Hsuff Hpref. iRevert (b'' Hsuff Hpref).
+      iInduction b' as [|[k'' x] b'] "IH".
+      - iIntros. wp_rec. wp_match. iFrame. by iLeft.
+      - iIntros (b'') "% %". rename_last Hpref. simplify_eq. simpl.
+        pose proof (proj1 (Forall_lookup _ _) HHKeys _ _ Hb) as HKeysb.
+        rewrite ->Forall_app, Forall_cons in HKeysb.
+        destruct HKeysb as [? [[k''' Hkey'] ?]].
+        wp_rec. wp_match. wp_proj. wp_proj. wp_lam. do 2 wp_proj. wp_lam. wp_proj. wp_lam.
+        wp_bind (equalf _ _). iApply wp_wand. by iApply equal_spec.
+        iIntros (?) "%". simplify_eq.
+        case_bool_decide.
+        + simplify_eq. wp_if. iPureIntro. right.
+          exists k'', x, b'.
+          rewrite /bucket_filter /filter /= decide_True ; last done.
+          rewrite decide_True ; eauto.
+        + assert (as_key k'' ≠ Some k).
+          rewrite Hkey'. injection. intros <-. contradiction.
+          wp_if. wp_bind ((rec: _ _ := _) _)%E. iApply (wp_wand with "[-]").
+          iApply ("IH" $! (b'' ++ [(k'', x)])).
+          iPureIntro. by rewrite -app_assoc.
+          iPureIntro. unfold bucket_filter in *. rewrite filter_app -Hpref /=.
+          by rewrite /filter /= decide_False. 
+          iIntros (?) "%". rename_last HInv.
+          decompose [and or ex] HInv. 
+          * simplify_eq. wp_match. rewrite /bucket_filter /filter /= decide_False ; eauto.
+          * simplify_eq/=. wp_match. do 2 wp_proj. iFrame. iRight. iPureIntro.
+            eexists _ , _ , ((_,_)::_).
+            rewrite /bucket_filter /filter /= decide_False ; last done.
+            rewrite decide_False ; eauto.
+    }
+    assert (HlookupData: lookup_data _ Hash data k = b) by by rewrite /lookup_data Hdata_refs Hb.
+    
+    case_eq (m !! k) ; [intros [|x ?] Hx | intros HNone] ;
+      [destruct (Hwf _ _ Hx) as [? [? ?]] ; discriminate |..] ;
+      last (iDestruct "HQ" as "[HQ' _]" ; iDestruct ("HQ'" with "[%] HP") as "HQ'" ; try done ;
+            iDestruct (fupd_mask_mono _ (⊤ ∖ ↑N.@0) with "HQ'") as ">[HP HQ']" ; try solve_ndisj).
+    all: iMod ("HClose" with "[Harr HP Hr2 Hrbs]") as "_" ;
+      try (iDestruct ("Hrbs" with "Hr2") as "?" ; iFrame ; iExists m, data ; iFrame ; eauto).
+    all: iModIntro ; wp_bind ((rec: _ _ := _) (bucket _))%E ; iApply (wp_wand with "Hloop") ;
+      iIntros (?) "%" ; rename_last HInv ;
+      destruct HInv as [[-> Hfilt] | [x' [k'' [? [? [Hfilt [-> ->]]]]]]].
+
+    all: destruct Hcontent as [Hin Hnin] ; try specialize (Hin _ _ Hx) ; try specialize (Hnin _ HNone).
+    all: try rewrite Hin HlookupData Hfilt /= in Hx ; try destruct (Hwf _ _ Hx) as [? [? ?]].
+    all: try by rewrite -HlookupData -Hnin in Hfilt.
+    - wp_lam. wp_match. wp_proj. wp_bind (_ <- _)%E.
+      iInv (N.@0) as "[Harr Hrest]" "HClose". clear dependent m data.
+      iDestruct "Hrest" as (m data) "[>% [>% [>% [>% [>% [HP Hrbs]]]]]]".
+      rename_last Hdata_refs. rename_last HHKeys. rename_last HNG. rename_last Hcontent.
+      assert (is_Some (data !! (Hash k `mod` length refs))) as [b' Hb'].
+      { apply lookup_lt_is_Some. rewrite Hdata_refs.
+        apply mod_bound_pos. lia. done. }
+      rewrite -{1}(take_drop_middle _ _ _ Hb') -{7}(take_drop_middle _ _ _ Hr).
+      repeat rewrite zip_with_app. repeat rewrite zip_with_cons.
+      iDestruct (big_sepL_app with "Hrbs") as "[Htake Hdrop]".
+      iDestruct (big_sepL_cons with "Hdrop") as "[>Hr2 Hdrop]".
+      iDestruct (mapsto_agree with "Hr2 Hr1") as "%".
+      rename_last HbEq. apply (inj bucket) in HbEq. simplify_eq.
+      iDestruct (fractional_half_2 with "Hr1 Hr2") as "Hr". apply _. wp_store.
+      iDestruct "Hr" as "[Hr1 Hr2]".
+      iDestruct "HQ" as "[_ HQ]". iDestruct ("HQ" with "[%] HP") as "HQ".
+      { assert (HlookupData: lookup_data _ Hash data k = b).
+        rewrite /lookup_data Hdata_refs Hb' //.
+        destruct Hcontent as [Hin Hnin]. case_eq (m !! k).
+        - intros ? Hlookup. rewrite (Hin _ _ Hlookup) HlookupData Hfilt //.
+        - intros Hn. rewrite -HlookupData -(Hnin _ Hn) // in Hfilt.
+      }
+      iDestruct (fupd_mask_mono _ (⊤ ∖ ↑N.@0) with "HQ") as ">[HP HQ]". solve_ndisj.
+      iMod ("HClose" with "[-Hr1 HΦ Hlocked HQ]") as "_".
+      {
+        iFrame. iNext.
+        iExists (remove_val m k),
+        (<[Hash k mod length data := bucket_remove _ _ _ k (lookup_data _ _ data k)]>data).
+        iSplit. iPureIntro. by apply table_wf_remove_val.
+        iSplit. iPureIntro. eapply content_remove ; try first [done | apply _ | lia].
+        iSplit. iPureIntro. by apply no_garbage_remove.
+        iSplit. iPureIntro. by apply have_keys_remove.
+        iSplit. iPureIntro. by rewrite /insert_data insert_length.
+        erewrite <-(take_drop_middle (<[_ := _]> _)).
+        rewrite /insert_data take_insert ; last reflexivity.
+        rewrite drop_insert ; last lia.
+        rewrite -{12}(take_drop_middle _ _ _ Hr).
+        repeat rewrite zip_with_app. repeat rewrite zip_with_cons.
+        rewrite big_sepL_app big_sepL_cons Hdata_refs.
+        iFrame.
+        rewrite 2!take_length Hdata_refs //.
+        rewrite /insert_data /lookup_data Hdata_refs.
+        rewrite Hb' /= list_lookup_insert. done.
+        rewrite Hdata_refs. apply mod_bound_pos ; [lia|done].
+      }
+      iModIntro. wp_lam.
+      wp_apply (release_spec with "[Hlocked Hr1]"). iFrame "Hlock Hlocked". eauto.
+      iIntros "_". wp_lam. wp_proj. iApply "HΦ". eauto.
+      rewrite 2!take_length Hdata_refs //.
+    - wp_lam. wp_match. wp_apply (release_spec with "[$Hlock $Hlocked Hr1]").
+      eauto. iIntros "_". wp_lam. iApply "HΦ". iLeft. eauto.
+      Unshelve. exact #().
+  Qed.
+  
+(*  Lemma table_remove_spec N P Q Q' k k' t:
+    as_key k' = Some k ->
+    {{{is_table N P t ∗
+       (∀ M,
+         ⌜head (lookup_all M k) = None⌝ -∗ P M ={⊤∖↑N}=∗ P M ∗ Q') ∧
+       ∀ M x,
+         ⌜head (lookup_all M k) = Some x⌝ -∗ P M ={⊤∖↑N}=∗ P (remove_val M k) ∗ Q k x}}}
+      table_remove t k'
+      {{{v x, RET v; ⌜v = NONEV⌝ ∗ Q' ∨ (⌜v = SOMEV x⌝ ∗ Q k x)}}}.
+  Proof.
+    iIntros (HKey Φ) "[HTable HQ] HΦ".
     iDestruct "HTable" as (arr refs locks γs) "[% [% [% [% [#Hlocks #HInv]]]]]".
     rename_last Hrefs_γs. rename_last Hrefs_locks. simplify_eq.
     do 2 wp_lam. wp_proj. wp_lam. wp_proj. wp_lam.
@@ -714,7 +908,8 @@ Section hashtable.
     assert (HlookupData: lookup_data _ Hash data k = b) by by rewrite /lookup_data Hdata_refs Hb'.
     
     case_eq (head (lookup_all M k)) ; [intros x Hx | intros HNone] ;
-      last iDestruct ("HQ'" with "[%] HP") as "[HP HQ']" ; try done.
+      last (iDestruct "HQ" as "[HQ' _]" ; iDestruct ("HQ'" with "[%] HP") as "HQ'" ; try done ;
+            try iDestruct (fupd_mask_mono _ (⊤ ∖ ↑N.@0) with "HQ'") as ">[HP HQ']" ; try solve_ndisj).
     all: iMod ("HClose" with "[Harr HP HrPtr Hpart Hrbγs]") as "_" ;
       try (iDestruct ("Hrbγs" with "[$HrPtr $Hpart]") as "?" ; iFrame ; iExists M, data ; iFrame ; eauto).
     all: iModIntro ; wp_bind ((rec: _ _ := _) (bucket _))%E ; iApply (wp_wand with "Hloop") ;
@@ -738,7 +933,7 @@ Section hashtable.
       iDestruct (table_own_eq with "[$Hpart $Hauth]") as "%". simplify_eq.
       wp_store.
       iDestruct (table_own_update _ _ (bucket_remove _ _ Hash k b) with "Hauth Hpart") as ">[Hauth Hpart]".
-      iFrame. iDestruct ("HQ" with "[%] HP") as "[HP HQ]".
+      iFrame. iDestruct "HQ" as "[_ HQ]". iDestruct ("HQ" with "[%] HP") as "HQ".
       { assert (HlookupData: lookup_data _ Hash data k = b).
         by rewrite /lookup_data Hdata_refs Hb'.
         unfold lookup_all. destruct Hcontent as [HSome HNone]. case_eq (M !! k).
@@ -746,6 +941,7 @@ Section hashtable.
         - intros Hn. erewrite <-(fmap_nil snd). erewrite (HNone _ Hn).
           by rewrite fmap_head HlookupData Hhead.
       }
+      iDestruct (fupd_mask_mono _ (⊤ ∖ ↑N.@0) with "HQ") as ">[HP HQ]". solve_ndisj.
       iMod ("HClose" with "[-Hauth HΦ Hlocked HQ]") as "_".
       {
         iFrame. iNext.
@@ -780,7 +976,7 @@ Section hashtable.
     - wp_lam. wp_match. wp_apply (release_spec with "[$Hlock $Hlocked Hauth]").
       eauto. iIntros "_". wp_lam. iApply "HΦ". iLeft. eauto.
       Unshelve. exact #().
-  Qed.
+  Qed.*)
    (* iMod ("HClose" with "[Harr HP HrPtr Hpart Hrbγs]") as "_".
     iDestruct ("Hrbγs" with "[$HrPtr $Hpart]") as "?". iFrame. iExists M, data. iFrame. eauto.
     iModIntro. wp_rec.
@@ -882,18 +1078,138 @@ Section hashtable.
       do 2 rewrite take_length. by rewrite(_:length data = length refs).
       Unshelve. exact #().
   Qed.*)
-  
+
   Lemma table_lookup_spec N P Q Q' k k' t:
     as_key k' = Some k ->
-    {{{is_table_alt N P t ∗
-       (∀ M,
-          ⌜head (lookup_all M k) = None⌝ -∗ P M -∗ P M ∗ Q') ∗
-       ∀ M x,
-         ⌜head (lookup_all M k) = Some x⌝ -∗ P M -∗ P M ∗ Q k x}}}
+    {{{is_table N P t ∗
+       (∀ m,
+          ⌜m !! k = None⌝ -∗ P m ={⊤∖↑N}=∗ P m ∗ Q') ∧
+       ∀ m x xs,
+         ⌜m !! k = Some (x :: xs)⌝ -∗ P m ={⊤∖↑N}=∗ P m ∗ Q k x}}}
       table_lookup t k'
       {{{v x, RET v; ⌜v = NONEV⌝ ∗ Q' ∨ (⌜v = SOMEV x⌝ ∗ Q k x)}}}.
   Proof.
-    iIntros (HKey Φ) "[HTable [HQ' HQ]] HΦ".
+    iIntros (HKey Φ) "[HTable HQ] HΦ".
+    iDestruct "HTable" as (arr refs locks) "[% [% [% [_ #Inv]]]]".
+    rename_last Hrefs_locks. simplify_eq.
+    do 2 wp_lam. wp_proj. wp_lam. wp_proj. wp_lam.
+    wp_bind (index _ _). iApply wp_wand. iApply index_spec. exact HKey.
+    iIntros (?) "%". simplify_eq.
+    wp_bind (array_load _).
+    iInv (N.@0) as "[Harr Hrest]" "HClose".
+    assert (is_Some (locks !! (Hash k `mod` length refs))) as [lk Hlk].
+    { apply lookup_lt_is_Some. rewrite -Hrefs_locks.
+      apply mod_bound_pos. lia. done. }
+    assert (is_Some (refs !! (Hash k `mod` length refs))) as [r Hr].
+    { apply lookup_lt_is_Some. apply mod_bound_pos. lia. done. }
+    wp_apply (array_load_spec _ _ (#r, lk) (Hash k `mod` length refs) with "Harr").
+    by rewrite lookup_zip_with list_lookup_fmap Hlk Hr.
+    iIntros "Harr". iMod ("HClose" with "[$Harr $Hrest]") as "_".
+    iModIntro. wp_proj. wp_bind (! _)%E.
+    iInv (N.@0) as "[Harr Hrest]" "HClose".
+    iDestruct "Hrest" as (m data) "[>% [>% [>% [>% [>% [HP Hrbs]]]]]]".
+    rename_last Hdata_refs. rename_last HHKeys. rename_last HNG. rename_last Hcontent. rename_last Hwf.
+    assert (is_Some (data !! (Hash k `mod` length refs))) as [b Hb].
+    { apply lookup_lt_is_Some. rewrite (_:length data = length refs) ; last done.
+      apply mod_bound_pos. lia. done. }
+    iDestruct (big_sepL_lookup_acc _ _ _ (r, b) with "Hrbs") as "[Hr1 Hrbs]".
+    by erewrite lookup_zip_with, Hr, Hb.
+    wp_load.
+
+    iAssert
+      (WP (rec: "go" "b"
+           := match: "b" with
+                InjL <> => InjL #()
+              | InjR "kxb" =>
+                let: "k'" := Fst (Fst "kxb") in
+                let: "x" := Snd (Fst "kxb") in
+                let: "b" := Snd "kxb" in
+                if: (equalf k') "k'"
+                then InjR "x"
+                else "go" "b" end) 
+          (bucket b)
+          {{ v, ⌜v = InjLV #() ∧ bucket_filter Σ Key Hash k b = [] ∨
+                (∃ (x k'' : val) b',
+                    v = InjRV x ∧
+                    bucket_filter Σ Key Hash k b = (k'', x)::b')⌝ }})%I as "Hloop".
+    {
+      assert (Hsuff: b = [] ++ b) by done.
+      assert (Hpref: [] = bucket_filter _ _ Hash k []) by done.
+      revert Hsuff Hpref. generalize b at 2 3 4 5. generalize ([] : bucket_data) at 1 3.
+      intros b'' b' Hsuff Hpref. iRevert (b'' Hsuff Hpref).
+      iInduction b' as [|[k'' x] b'] "IH".
+      - iIntros. wp_rec. wp_match. by iLeft.
+      - iIntros (b'') "% %".
+        rename_last Hpref. simplify_eq.
+        pose proof (proj1 (Forall_lookup _ _) HHKeys _ _ Hb) as HKeysb.
+        rewrite ->Forall_app, Forall_cons in HKeysb.
+        destruct HKeysb as [? [[k''' Hkey'] ?]].
+        wp_rec. wp_match. repeat first [wp_proj | wp_lam].
+        wp_bind (equalf _ _). iApply wp_wand. by iApply equal_spec.
+        iIntros (?) "%". simplify_eq.
+        case_bool_decide.
+        + simplify_eq.          
+          wp_if. iPureIntro. right.
+          exists x, k''.
+          rewrite /bucket_filter /filter /= decide_True ; eauto.
+        + wp_if.
+          assert (as_key k'' ≠ Some k).
+          rewrite Hkey'. injection. intros <-. contradiction.
+          iApply (wp_wand with "[-]"). iApply ("IH" $! (b'' ++ [(k'', x)])).
+          iPureIntro. by rewrite -app_assoc.
+          iPureIntro. unfold bucket_filter in *. rewrite filter_app -Hpref /=.
+          by rewrite /filter /= decide_False. 
+          iIntros (?) "%". rename_last HInv.
+          decompose [and or ex] HInv. 
+          * simplify_eq. rewrite /bucket_filter /filter /= decide_False ; eauto.
+          * simplify_eq. iPureIntro. right.
+            eexists _ , _ .
+            rewrite /bucket_filter /filter /= decide_False ; eauto. 
+    }
+    assert (HlookupData: lookup_data _ Hash data k = b).
+    by rewrite /lookup_data Hdata_refs Hb.
+
+ (*   case_eq (m !! k) ; [intros [|x ?] Hx | intros HNone] ;
+      [destruct (Hwf _ _ Hx) as [? [? ?]] ; discriminate |..] ;
+      last (iDestruct "HQ" as "[HQ' _]" ; iDestruct ("HQ'" with "[%] HP") as "HQ'" ; try done ;
+            iDestruct (fupd_mask_mono _ (⊤ ∖ ↑N.@0) with "HQ'") as ">[HP HQ']" ; try solve_ndisj).
+    all: iMod ("HClose" with "[Harr HP HrPtr Hpart Hrbγs]") as "_" ;
+      try (iDestruct ("Hrbγs" with "[$HrPtr $Hpart]") as "?" ; iFrame ; iExists m, data ; iFrame ; eauto).
+    all: iModIntro ; wp_bind ((rec: _ _ := _) (bucket _))%E ; iApply (wp_wand with "Hloop") ;
+      iIntros (?) "%" ; rename_last HInv ;
+        destruct HInv as [[-> Hfilt] | [x' [k'' [? [? [Hfilt [-> ->]]]]]]].*)
+
+    case_eq (m !! k) ; [intros [|x ?] Hx | intros HNone] ;
+      [destruct (Hwf _ _ Hx) as [? [? ?]] ; discriminate |..] ;
+      [ iDestruct "HQ" as "[_ HQ]" | iDestruct "HQ" as "[HQ _]"] ;
+      iDestruct ("HQ" with "[%] HP") as "HQ" ; try done ;
+      iDestruct (fupd_mask_mono _ (⊤ ∖ ↑N.@0) with "HQ") as ">[HP HQ]" ; try solve_ndisj.
+    all: iMod ("HClose" with "[Harr HP Hr1 Hrbs]") as "_" ;
+      try (iDestruct ("Hrbs" with "Hr1") as "?" ; iFrame ; iExists m, data ; iFrame ; eauto).
+    all: iModIntro ; wp_lam ; iApply (wp_wand with "Hloop") ;
+      iIntros (?) "%" ; rename_last HInv ;
+      destruct HInv as [[-> Hfilt] | [x' [k'' [? [-> Hfilt]]]]] ; iApply "HΦ".
+
+    all: destruct Hcontent as [Hin Hnin] ;
+      first [specialize (Hin _ _ Hx) ; clear Hnin | specialize (Hnin _ HNone)].
+    all: try rewrite Hin HlookupData Hfilt /= in Hx ; try by destruct (Hwf _ _ Hx) as [? [? ?]].
+    all: try rewrite -HlookupData -Hnin // in Hfilt.
+    - rewrite HlookupData Hfilt in Hin. injection Hin as ->. eauto.
+    - eauto. 
+    Unshelve. all: exact #().
+  Qed.
+  
+ (* Lemma table_lookup_spec N P Q Q' k k' t:
+    as_key k' = Some k ->
+    {{{is_table_alt N P t ∗
+       (∀ M,
+          ⌜head (lookup_all M k) = None⌝ -∗ P M ={⊤∖↑N}=∗ P M ∗ Q') ∧
+       ∀ M x,
+         ⌜head (lookup_all M k) = Some x⌝ -∗ P M ={⊤∖↑N}=∗ P M ∗ Q k x}}}
+      table_lookup t k'
+      {{{v x, RET v; ⌜v = NONEV⌝ ∗ Q' ∨ (⌜v = SOMEV x⌝ ∗ Q k x)}}}.
+  Proof.
+    iIntros (HKey Φ) "[HTable HQ] HΦ".
     iDestruct "HTable" as (arr refs locks γs) "[% [% [% [% [_ #Inv]]]]]".
     rename_last Hrefs_γs. rename_last Hrefs_locks. simplify_eq.
     do 2 wp_lam. wp_proj. wp_lam. wp_proj. wp_lam.
@@ -977,7 +1293,9 @@ Section hashtable.
     by rewrite /lookup_data Hdata_refs Hb.
     
     case_eq (head (lookup_all M k)) ; [intros x Hx | intros HNone] ;
-      [iDestruct ("HQ" with "[%] HP") as "[HP HQ]" | iDestruct ("HQ'" with "[%] HP") as "[HP HQ']"] ; try done.
+      [ iDestruct "HQ" as "[_ HQ]" | iDestruct "HQ" as "[HQ _]"] ;
+      iDestruct ("HQ" with "[%] HP") as "HQ" ; try done ;
+      iDestruct (fupd_mask_mono _ (⊤ ∖ ↑N.@0) with "HQ") as ">[HP HQ]" ; try solve_ndisj.
     all: iMod ("HClose" with "[Harr HP HrPtr Hpart Hrbγs]") as "_" ;
       try (iDestruct ("Hrbγs" with "[$HrPtr $Hpart]") as "?" ; iFrame ; iExists M, data ; iFrame ; eauto).
     all: iModIntro ; wp_lam ; iApply (wp_wand with "Hloop") ;
@@ -990,8 +1308,8 @@ Section hashtable.
     - injection Hx as ->. eauto.
     - eauto. 
     Unshelve. all: exact #().
-  Qed.
-
+  Qed.*)
+(*
   Lemma lookup_union_None_l `{FinMap K C} {A} (m1 m2 : C A) i :
     m1 !! i = None -> (m1 ∪ m2) !! i = m2 !! i.
   Proof.
@@ -1210,7 +1528,8 @@ Section hashtable.
     lookup_all M k = [] -> cleanup_table M !! k = None.
   Proof. rewrite /lookup_all lookup_omap. by destruct (M !! k) as [[|?]|]. Qed.
 
-  Lemma table_fold_spec N P (Q : Map (list val) -> set Key -> iProp Σ) I (f t a : val) :
+  Lemma table_fold_spec N P (Q : Map (list val) -> set Key -> iProp Σ)
+        (I : list (val * val) → val → iProp Σ) (f t a : val) :
     Proper ((MEquiv) ==> (≡) ==> (⊣⊢)) Q ->
     (forall M M1 M2 D D1 D2,
         M1 ⊥ₘ M2 -> M = M1 ∪ M2 ->
@@ -1223,15 +1542,24 @@ Section hashtable.
         {{⌜permitted M (seq ++ [(k, x)])⌝ ∗ Q M D ∗ I seq a}}
           f k x a
         {{v, Q M D ∗ I (seq ++ [(k, x)]) v}}) -∗
-    {{{is_table_alt N P t ∗ Q ∅ ∅ ∗ I [] a}}}
+    {{{is_table_alt N P t ∗ I [] a}}}
       table_fold f t a
     {{{v M seq, RET v ; Q M ⊤ ∗ ⌜complete M seq⌝ ∗ I seq v}}}.
   Proof.
     iIntros (HProper HQsplit) "#HPQ #Hf !#".
-    iIntros (Φ) "[#HTable [HQ HI]] HΦ".
+    iIntros (Φ) "[#HTable HI] HΦ".
     iDestruct "HTable" as (arr refs locks γs) "[% [% [% [% [_ #Inv]]]]]".
     rename_last Hrefs_γs. rename_last Hrefs_locks. simplify_eq.
-    do 3 wp_lam.
+    iApply fupd_wp.
+    iMod (inv_open with "Inv") as "[[Harr Hrest] HClose]". solve_ndisj.  
+    iDestruct "Hrest" as (M data) "[? [? [? [? [HP Hrbγs]]]]]".
+    iDestruct ("HPQ" with "HP") as "[HP HQ]".
+    rewrite (HQsplit M M ∅ _ ⊤ ∅) ; first last.
+    intros. apply lookup_empty. done. rewrite right_id //.
+    apply disjoint_empty_r. rewrite right_id //. apply map_disjoint_empty_r.
+    iDestruct "HQ" as "[_ HQ]".
+    iMod ("HClose" with "[-HQ HI HΦ]") as "_". iFrame. iExists M, data. iFrame.
+    clear M data. iModIntro. do 3 wp_lam.
     iDestruct (table_fold_inv_init Q (length refs) HProper with "HQ") as "HInv".
     rewrite -inj_0.
     generalize 0 at 2 3, (@nil (val * val)) at 3 4, (∅ : Map (list val)).
@@ -1340,6 +1668,6 @@ Section hashtable.
       apply mod_bound_pos ; lia. trans (length refs). apply mod_bound_pos ; lia. lia.
   Qed.
            
-          
+          *)
           
 End hashtable.
