concurrent/partial_table_use.v
@@ -1,48 +1,232 @@
+From stdpp Require Import bset.
 From iris.proofmode Require Import tactics.
 From iris.algebra Require Import auth.
+From iris.program_logic Require Import hoare.
 From iris.heap_lang.lib Require Import lock.
+From iris_programs Require Import array.
 From iris_programs.concurrent Require Import hashtable partial.
-
-Ltac rename_last H' := match goal with [H : _ |- _] => rename H into H' end ; move H' at top.
+From iris_programs.iterators Require Import util.
 
 Instance partial_table_auth_discrete M K `{FinMap K M} V : CMRADiscrete (authR (partial_tableUR K V M)).
 Proof. apply _. Qed.
 Class partialG M K `{FinMap K M} V Σ := {partial_inG :> inG Σ (authR (partial_tableUR K V M))}.
 Section derived.
-  Context Map Key `{FinMap Key Map}.
-  Context Σ Hash `{!heapG Σ} `{!Hashable Σ Key Hash} `{!Array Σ} `{!tableG Σ} `{!partialG Map Key val Σ}.
+  Context map key Σ hash `{FinMap key map} `{!heapG Σ} `{!Hashable Σ key hash} `{!Array Σ} `{!partialG map key val Σ}.
   Variable lck : lock Σ.
-  Variable modulo: val.
-  Hypothesis modulo_spec:
-    forall (m n : Z), WP modulo (#m, #n) {{v, ⌜v = #(m `mod` n)⌝}}%I.
-  Definition partial_inv γ M : iProp Σ := own γ (● PTCar (M, ⊤)).
-  Definition partial_own γ M d : iProp Σ := own γ (◯ PTCar (M, d)).
+  Definition partial_inv γ m : iProp Σ := own γ (● PTCar (m, ⊤)).
+  Definition partial_own γ m d : iProp Σ := own γ (◯ PTCar (m, d)).
 
-  Lemma own_partial_table_lookup γ M M' d k :
+  Lemma own_partial_table_lookup γ m m' d k :
     k ∈ d ->
-    (partial_inv γ M ∗ partial_own γ M' d → ⌜M !! k = M' !! k⌝)%I.
+    (partial_inv γ m ∗ partial_own γ m' d → ⌜m !! k = m' !! k⌝)%I.
   Proof.
     intro Hin. rewrite -own_op. iIntros "Hown".
     iDestruct (own_valid with "Hown") as "Hval". rewrite uPred.discrete_valid.
     iDestruct "Hval" as "%". rename_last Hval. iPureIntro.
-    rewrite -(lookup_cut_table_elem_of M d) // -(partial_table_included_cut_table M' _ _ ⊤) //.
+    rewrite -(lookup_cut_table_elem_of m d) // -(partial_table_included_cut_table m' _ _ ⊤) //.
     split. apply multiset_top_no_dup. eauto.
     apply auth_valid_discrete_2 in Hval. by destruct Hval.
   Qed.
+
+  Lemma partial_table_create_spec N (n : nat):
+    n > 0 ->
+    WP create_table Σ lck #n
+       {{t, ∃ γ, is_table Σ key hash map lck N (partial_inv γ) t ∗ partial_own γ ∅ ⊤}}%I.
+  Proof.
+    intro. iMod (own_alloc (● PTCar (∅, ⊤) ⋅ ◯ PTCar (∅, ⊤))) as (γ) "[Hinv Hown]".
+    apply auth_valid_discrete_2. split. done. split. apply multiset_top_no_dup. done.
+    iApply (create_table_spec _ _ _ _ _ _ (partial_inv γ) with "Hinv"). done.
+    iNext. iIntros. iExists (γ). iFrame "#". iFrame.
+  Qed.
   
-  Lemma table_insert_spec N γ M d k k' x t:
+  Lemma partial_table_insert_spec N γ m d k k' x t:
     as_key k' = Some k ->
     k ∈ d ->
-    {{{is_table_alt Σ Key Hash Map lck N (partial_inv γ) t ∗ partial_own γ M d }}}
-      (table_insert Σ Key Hash lck modulo) t k' x
-    {{{RET #(); partial_own γ (insert_val M k x) d}}}.
+    {{{is_table Σ key hash map lck N (partial_inv γ) t ∗ partial_own γ m d }}}
+      (table_insert Σ key hash lck) t k' x
+    {{{RET #(); partial_own γ (insert_val m k x) d}}}.
   Proof.
     intros Hkey Hin. iIntros (Φ) "[#Htable Hown] HΦ".
-    iApply (table_insert_spec2 with "[$Htable Hown]"). done. done.
-    iIntros (M') "Hinv". unfold insert_val, lookup_all.
+    iApply (table_insert_spec with "[$Htable Hown]") ; try done.
+    iIntros (m') "Hinv". unfold insert_val.
     iDestruct (own_partial_table_lookup with "[$Hown $Hinv]") as "%". done.
     rename_last Heq. rewrite Heq.
     iApply own_op. iApply bupd_fupd. iApply own_update.
     apply auth_update, partial_table_local_update_partial_alter. done.
-    iSplitL "Hinv" ; iFrame. iApply "HΦ".
+    iSplitL "Hinv" ; iFrame.
   Qed.
+
+  Lemma table_lookup_spec N γ m d k k' t:
+    as_key k' = Some k ->
+    k ∈ d ->
+    {{{is_table Σ key hash map lck N (partial_inv γ) t ∗ partial_own γ m d }}}
+      (table_lookup Σ key hash) t k'
+    {{{RET match m !! k with
+             Some (v :: _) => SOMEV v
+           | _ => NONEV end ;
+       partial_own γ m d}}}.
+  Proof.
+    intros Hkey Hin. iIntros (Φ) "[#Htable Hown] HΦ". About table_lookup_spec.
+    iApply (table_lookup_spec _ _ _ _ _ _ _
+                              (fun _ x => (∃ xs, ⌜m !! k = Some (x :: xs)⌝) ∗ partial_own γ m d)%I
+                              (⌜m !! k = None⌝ ∗ partial_own γ m d)%I
+              with "[$Htable Hown]") ; try done.
+    iSplit ; [iIntros (m' Hlookup) | iIntros (m' x xs Hlookup)] ; iIntros "Hinv !>" ;
+      iDestruct (own_partial_table_lookup with "[$Hown $Hinv]") as "%" ; try done ;
+      rename_last Heq ; rewrite Heq in Hlookup ; iFrame ; eauto.
+    iNext.
+    iIntros (? ?) "[[% [% ?]]|[% [Hex ?]]]" ; last iDestruct "Hex" as (?) "%" ;
+      simplify_eq ; rename_last Hlookup ; rewrite Hlookup ;
+      iApply "HΦ" ; iFrame.
+  Qed.
+
+  Lemma table_remove_spec N γ m d k k' t:
+    as_key k' = Some k ->
+    k ∈ d ->
+    {{{is_table Σ key hash map lck N (partial_inv γ) t ∗ partial_own γ m d }}}
+      (table_remove Σ key hash lck) t k'
+    {{{RET match m !! k with
+             Some (v :: _) => SOMEV v
+           | _ => NONEV end ;
+       partial_own γ (remove_val m k) d}}}.
+  Proof.
+    intros Hkey Hin. iIntros (Φ) "[#Htable Hown] HΦ".
+    iApply (table_remove_spec _ _ _ _ _ _ _
+                               (fun _ x =>
+                                  (∃ xs, ⌜m !! k = Some (x :: xs)⌝) ∗
+                                  partial_own γ (remove_val m k) d)%I
+                               (⌜m !! k = None⌝ ∗
+                                 partial_own γ m d)%I
+              with "[$Htable Hown]") ; try done.
+    {
+      iSplit ; [iIntros (m' Hlookup) | iIntros (m' ? x Hlookup) ] ; iIntros "Hinv" ;
+        iDestruct (own_partial_table_lookup with "[$Hown $Hinv]") as "%";
+        try done ; rename_last Heq ; rewrite Heq in Hlookup.
+      - iFrame. done.
+      - rewrite [(_ ∗ partial_own _ _ _)%I]comm assoc. iSplitL ; last eauto.
+        iApply own_op. iApply bupd_fupd. iApply own_update.
+        rewrite /remove_val Heq Hlookup.
+        apply auth_update. destruct x ; by apply partial_table_local_update_partial_alter.
+        iApply own_op. iFrame.
+    }
+    iNext.
+    iIntros (? ?) "[[% [% ?]]|[% [% ?]]]" ; simplify_eq ;
+      rename_last Hlookup ; last destruct Hlookup as [? Hlookup] ;
+      rewrite /remove_val Hlookup ; iApply "HΦ" ; iFrame.
+  Qed.   
+(*
+  Hypothesis table_fold_spec2
+    : ∀ (N : namespace) (P : Map (list val) → uPred (iResUR Σ))
+        (Q : Map (list val) → bset Key -> iProp Σ)
+           (I : list (val * val) → val → iProp Σ) (f t a : val),
+           Proper ((=) ==> equiv ==> equiv) Q
+           → (∀ (M M1 M2 : Map (list val)) (D D1 D2 : bset Key),
+              M1 ⊥ₘ M2
+              → M = M1 ∪ M2
+                → D1 ⊥ D2
+                  → D ≡ D1 ∪ D2
+                    → (∀ k : Key, k ∉ D1 → M1 !! k = None)
+                      → (∀ k : Key, k ∉ D2 → M2 !! k = None) → Q M D ≡ (Q M1 D1 ∗ Q M2 D2)%I)
+             → □ (∀ M : Map (list val), P M -∗ P M ∗ Q M ⊤) -∗
+               (∀ (M : Map (list val)) (D : bset Key) (seq : list (val * val)) (k x a0 : val),
+                {{ ⌜permitted M (seq ++ [(k, x)])⌝ ∗ Q M D ∗ I seq a0 }} ((f k) x) a0 {{ v, 
+                Q M D ∗ I (seq ++ [(k, x)]) v }}) -∗
+               {{{ is_table_alt Σ Key Hash Map lck N P t ∗ I [] a }}} (((table_fold Σ) f) t) a {{{ 
+               (v : val)(M : Map (list val))(seq : list (val * val)),  RET v; Q M ⊤
+                                                                                ∗ ⌜complete M seq⌝ ∗ I seq v}}}.
+
+  Definition multiset_of_bset {A} (X : bset A) : multiset A := {[x | x ∈ X]}.
+  Instance multiset_of_bset_proper {A} : Proper ((≡) ==> (≡)) (@multiset_of_bset A).
+  Proof.
+    intros ?? Heq x. rewrite /multiset_of_bset /=. case_decide as Hin ; rewrite ->Heq in Hin.
+    - rewrite decide_True //.
+    - rewrite decide_False //.
+  Qed.
+
+  Lemma multiset_of_bset_elem_of {A} (X : bset A) x :
+    x ∈ multiset_of_bset X ↔ x ∈ X.
+  Proof.
+    rewrite {1}/elem_of /multiset_elem_of /=. by case_decide.
+  Qed.
+
+  Lemma cut_table_disjoint (m1 m2 : Map (list val)) d1 d2 :
+    d1 ⊥ d2 -> cut_table d1 m1 ⊥ₘ cut_table d2 m2. 
+  Proof.
+    rewrite elem_of_disjoint. intro Hdisj.
+    apply map_disjoint_spec. intros k ?? Hlookup1 Hlookup2.
+    destruct (decide (k ∈ d1)). destruct (decide (k ∈ d2)).
+    - by eapply Hdisj.
+    - rewrite lookup_cut_table_not_elem_of // in Hlookup2.
+    - rewrite lookup_cut_table_not_elem_of // in Hlookup1.
+  Qed.
+    
+  Lemma table_fold_spec N γ M I (f t a : val) :
+    ((∀ k x seq (a : val),
+         {{⌜permitted M (seq ++ [(k, x)])⌝ ∗ I seq a}}
+           f k x a
+         {{v,I (seq ++ [(k ,x)]) v }}) -∗
+    {{{is_table_alt Σ Key Hash Map lck N (partial_inv γ) t ∗ partial_own γ M ⊤ ∗ I [] a}}}
+      table_fold Σ f t a
+    {{{v seq, RET v; ⌜complete M seq⌝ ∗
+                     is_table_alt Σ Key Hash Map lck N (partial_inv γ) t ∗
+                     partial_own γ M ⊤ ∗ I seq v}}})%I.
+  Proof.
+    iIntros "#Hf !#". iIntros (Φ) "[#Htable Hown] HΦ".
+    Check table_fold_spec2.
+    iApply (table_fold_spec2 N (partial_inv γ)
+                            (fun M' d' =>
+                               □(partial_own γ M ⊤ →
+                                 ⌜M' = cut_table (multiset_of_bset d') M⌝))%I
+                            (fun seq a => partial_own γ M ⊤ ∗ I seq a)%I
+                            f t a).
+    { intros ?? <- ?? Heq. pose proof (@cut_table_proper). rewrite Heq //. }
+    { intros m m1 m2 d d1 d2 Hmdisj -> Hddisj Hdunion Hdom1 Hdom2. iSplit.
+      - iIntros "#Himpl" ; iSplit ; iIntros "!# Hown" ; iDestruct ("Himpl" with "Hown") as %Heq ;
+        iPureIntro ; apply map_eq ; intro k.
+        + destruct (decide (k ∈ d1)).
+          * rewrite lookup_cut_table_elem_of ; last by apply multiset_of_bset_elem_of.
+            rewrite -(lookup_cut_table_elem_of M (multiset_of_bset d)) ; last first.
+            apply multiset_of_bset_elem_of. rewrite Hdunion. apply elem_of_union. by left.
+            rewrite <-Heq. case_eq (m1 !! k).
+            -- symmetry. by apply lookup_union_Some_l.
+            -- symmetry. apply lookup_union_None. split. done. apply Hdom2.
+               intro. rewrite ->elem_of_disjoint in Hddisj. by eapply Hddisj.
+          *  rewrite lookup_cut_table_not_elem_of. by apply Hdom1. rewrite multiset_of_bset_elem_of //.
+        + destruct (decide (k ∈ d2)).
+          * rewrite lookup_cut_table_elem_of ; last by apply multiset_of_bset_elem_of.
+            rewrite -(lookup_cut_table_elem_of M (multiset_of_bset d)) ; last first.
+            apply multiset_of_bset_elem_of. rewrite Hdunion. apply elem_of_union. by right.
+            rewrite <-Heq. case_eq (m2 !! k).
+            -- symmetry. by apply lookup_union_Some_r.
+            -- symmetry. apply lookup_union_None. split ; last done. apply Hdom1.
+               intro. rewrite ->elem_of_disjoint in Hddisj. by eapply Hddisj.
+          *  rewrite lookup_cut_table_not_elem_of. by apply Hdom2. rewrite multiset_of_bset_elem_of //.
+      - iIntros "[#Himpl1 #Himpl2] !# Hown".
+        iDestruct ("Himpl1" with "Hown") as %->.
+        iDestruct ("Himpl2" with "Hown") as %->.
+        iPureIntro. apply map_eq. intro k. destruct (decide (k ∈ d1)).
+        + rewrite lookup_cut_table_elem_of ; last first.
+          apply multiset_of_bset_elem_of. rewrite Hdunion. apply elem_of_union. by left.
+          case_eq (M !! k).
+          * intros. apply lookup_union_Some_l. rewrite lookup_cut_table_elem_of //.
+            by apply multiset_of_bset_elem_of. 
+          * intros. apply lookup_union_None. split.
+            -- rewrite lookup_cut_table_elem_of //. by apply multiset_of_bset_elem_of.
+            -- apply Hdom2. intro. rewrite ->elem_of_disjoint in Hddisj. by eapply Hddisj. 
+        + destruct (decide (k ∈ d2)).
+          * rewrite lookup_cut_table_elem_of ; last first.
+            apply multiset_of_bset_elem_of. rewrite Hdunion. apply elem_of_union. by right.
+            case_eq (M !! k).
+            -- intros. apply lookup_union_Some_r. apply cut_table_disjoint, elem_of_disjoint. intro.
+               rewrite 2!multiset_of_bset_elem_of. apply Hddisj.
+               rewrite lookup_cut_table_elem_of // multiset_of_bset_elem_of //.
+            -- intros. apply lookup_union_None. split.
+               ++ by apply Hdom1.
+               ++ rewrite lookup_cut_table_elem_of // multiset_of_bset_elem_of //.
+          * rewrite lookup_cut_table_not_elem_of. apply lookup_union_None. eauto.
+            rewrite multiset_of_bset_elem_of Hdunion elem_of_union. intuition.
+    }
+    { iIntros "!#". iIntros (m) "Hinv". iSplit. iFrame. iApply persistentP. . iIntros "!# Hown".
+ *)
+
+End derived.
