iterators/hashtable_model.v
@@ -16,21 +16,57 @@ Class Hashable Σ `{heapG Σ} (Key : Type) `{EqDecision Key} (Hash : Key -> nat)
     hash_spec k v : as_key v = Some k -> WP hashf v {{u, ⌜u = #(Hash k)⌝}}%I }.
 
 Section model.
-  Context `{Hashable Σ Key Hash}.
-  Context `{FinMap Key Map}.
-  
-  Implicit Type M : Map (list val).
-  
-  
-  Definition lookup_all M k := from_option id [] (M !! k).
-  
-  Definition insert_val M k x := (<[k := x :: lookup_all M k]>M).
-  
-  Definition remove_val M k := (<[ k := tail (lookup_all M k)]>M).
+  Context {Σ Key Hash map} `{FinMap Key map, heapG Σ, !Hashable Σ Key Hash}.
 
-  Definition all_elements M := map_fold (fun k l acc => ((fun v => (k, v)) <$> l) ++ acc) [] M.
+  Implicit Type m : map (list val).
   
-  Definition MEquiv (M1 M2 : Map (list val)) : Prop := forall k, lookup_all M1 k = lookup_all M2 k.
+  
+ (* Definition lookup_all m k := from_option id [] (m !! k).*)
+  
+  Definition insert_val m k x := (<[k := x :: from_option id [] (m !! k)]>m).
+  
+  Definition remove_val m k := match m !! k with
+                               | Some (x :: y :: l) => <[k := y :: l]> m
+                               | Some _ => delete k m
+                               | None => m
+                               end.
+
+                                 (*(<[ k := tail (lookup_all M k)]>M).*)
+
+  Definition all_elements m := map_fold (fun k l acc => ((fun v => (k, v)) <$> l) ++ acc) [] m.
+
+  Definition table_wf m := map_Forall (fun _ l => exists x xs, l = x :: xs) m.
+
+  Lemma table_wf_empty : table_wf ∅.
+  Proof. apply map_Forall_empty. Qed.
+  
+  Lemma table_wf_insert_val m k x : table_wf m -> table_wf (insert_val m k x).
+  Proof. apply map_Forall_insert_2. eauto. Qed.
+
+  Lemma table_wf_remove_val m k : table_wf m -> table_wf (remove_val m k).
+  Proof.
+    unfold remove_val.
+    case_eq (m !! k) ; last done.
+    intros [|?[|]] Hlookup ; last (apply map_Forall_insert_2 ; eauto).
+    all: rewrite -{1}(insert_id _ _ _ Hlookup) -insert_delete ;
+      apply map_Forall_insert_12, lookup_delete.
+  Qed.
+
+  Definition lookup_insert_val_ne m k k' x :
+    k ≠ k' -> (insert_val m k x) !! k' = m !! k'. 
+  Proof.
+    intros Hne. rewrite /insert_val lookup_insert_ne //.
+  Qed.
+  
+  Definition lookup_remove_val_ne m k k' :
+    k ≠ k' -> (remove_val m k) !! k' = m !! k'. 
+  Proof.
+    intros Hne. unfold remove_val.
+    case_eq (m !! k) ; last done.
+    intros [|?[|]] Hlookup ; [apply lookup_delete_ne ..| apply lookup_insert_ne] ; done.
+  Qed.
+  
+(*  Definition MEquiv (m1 m2 : Map (list val)) : Prop := forall k, lookup_all m1 k = lookup_all m2 k.
   
   Global Instance MEquiv_equivalence : Equivalence MEquiv.
   Proof. split. by intros ??.
@@ -44,7 +80,7 @@ Section model.
 
   Global Instance insert_proper : Proper ((=) ==> (=) ==> MEquiv ==> MEquiv) insert.
   Proof.
-    intros k? <- x? <- M1 M2 Heq k'.
+    intros k? <- x? <- m1 m2 Heq k'.
       rewrite /lookup_all /insert_val. destruct (decide (k = k')) as [<-|].
     - do 2 rewrite lookup_insert.  reflexivity.
     - do 2 (rewrite lookup_insert_ne ; last assumption). apply Heq.
@@ -53,40 +89,40 @@ Section model.
   
   Global Instance insert_val_proper : Proper (MEquiv ==> (=) ==> (=) ==> MEquiv) insert_val.
   Proof.
-    intros M1 M2 Heq k? <- x? <- k'.
+    intros m1 m2 Heq k? <- x? <- k'.
       rewrite  /insert_val insert_proper ; [reflexivity..|by rewrite Heq |assumption].
   Qed.
   
-  Global Instance remove_val_proper : Proper (MEquiv ==> (=) ==> MEquiv) remove_val.
+(*  Global Instance remove_val_proper : Proper (MEquiv ==> (=) ==> MEquiv) remove_val.
   Proof.
-    intros M1 M2 Heq k? <- k'.
+    intros m1 m2 Heq k? <- k'.
     rewrite /remove_val insert_proper ; [reflexivity..|by rewrite Heq | assumption].
-  Qed.
+  Qed. *)
 
   Lemma table_ind :
     forall (P : Map (list val) -> Prop),
     Proper ( MEquiv ==> (↔)) P ->
-    P ∅ -> (∀ k x M, P M → P (insert_val M k x)) → ∀ M, P M.
+    P ∅ -> (∀ k x m, P m → P (insert_val m k x)) → ∀ m, P m.
   Proof.
-    intros P ? Hempty Hind M.
-    induction M as [|k l M Hlookup IHM] using map_ind. assumption.
+    intros P ? Hempty Hind m.
+    induction m as [|k l m Hlookup IHm] using map_ind. assumption.
     induction l.
-    - rewrite (_:MEquiv (<[k:=[]]> M) M). assumption.
+    - rewrite (_:MEquiv (<[k:=[]]> m) m). assumption.
       intros k'. unfold lookup_all.
       destruct (decide (k = k')) as [<-|].
       + by rewrite Hlookup lookup_insert. 
       + by rewrite lookup_insert_ne.
     - unfold insert_val in Hind.
       rewrite -(insert_insert _ _ _ l).
-      rewrite {1}(_: l = lookup_all (<[k:=l]> M) k).
+      rewrite {1}(_: l = lookup_all (<[k:=l]> m) k).
       auto. by rewrite /lookup_all lookup_insert.
   Qed.      
 
-  Lemma MEquiv_proper `(R : relation B) (f : Key -> list val -> B -> B) fM `{!Equivalence R} :
+  Lemma MEquiv_proper `(R : relation B) (f : Key -> list val -> B -> B) fm `{!Equivalence R} :
     Proper ((=) ==> (=) ==> R ==> R) f -> 
-    (forall k l M, M !! k = None -> R (f k l (fM M)) (fM (<[k:=l]>M))) ->
-    (forall M k, R (f k [] (fM M)) (fM M))  ->
-    Proper (MEquiv ==> R) fM.
+    (forall k l m, m !! k = None -> R (f k l (fm m)) (fm (<[k:=l]>m))) ->
+    (forall m k, R (f k [] (fm m)) (fm m))  ->
+    Proper (MEquiv ==> R) fm.
   Proof.
     intros ? Hinsert Hnil M1. induction M1 as [|k l M1 Hlookup IH]  using map_ind.
     - intro M2. induction M2 as [|k l M2 Hlookup IH] using map_ind.
@@ -127,20 +163,20 @@ Section model.
     intros. unfold all_elements. erewrite (map_fold_insert Permutation). reflexivity. solve_proper.
     intros. do 2 rewrite app_assoc. f_equiv. apply Permutation_app_comm.
     assumption. reflexivity.
-  Qed.
+  Qed.*)
 
-  
-  Lemma insert_remove_val M k x:
-    MEquiv (remove_val (insert_val M k x) k) M.
+  (*
+  Lemma insert_remove_val m k x:
+    MEquiv (remove_val (insert_val m k x) k) m.
   Proof.
     rewrite /remove_val /insert_val insert_insert /lookup_all lookup_insert /=.
     intro k' ; unfold lookup_all ; destruct (decide (k = k')) as [<-|].
-    - destruct (M !! k) ; by rewrite lookup_insert.        
+    - destruct (m !! k) ; by rewrite lookup_insert.        
     - by rewrite lookup_insert_ne.
-  Qed.
-
-  Lemma lookup_insert_val M k x:
-    head (lookup_all M k) = Some x ↔ MEquiv (insert_val (remove_val M k) k x) M.
+  Qed.*)
+(*
+  Lemma lookup_insert_val m k x:
+    head (lookup_all m k) = Some x ↔ MEquiv (insert_val (remove_val m k) k x) m.
   Proof.
     split.
     - rewrite /insert_val /remove_val /lookup_all insert_insert lookup_insert. intro HSome.
@@ -148,9 +184,38 @@ Section model.
       intro k'. unfold lookup_all. destruct (decide (k = k')) as [<-|].
       by rewrite lookup_insert. by rewrite lookup_insert_ne.
     - intros <-. by rewrite /lookup_all /insert_val /remove_val lookup_insert.
+  Qed.*)
+
+  Inductive removal : map (list val) -> list (val * val) -> map (list val) -> Prop :=
+  | RemovalNil {m} : removal m [] m
+  | RemovalCons {k k' x xs l m m' } :
+      as_key k = Some k' ->
+      m !! k' = Some (x :: xs) ->
+      removal (remove_val m k') l m' ->
+      removal m ((k, x) :: l) m'.   
+    
+  Lemma removal_app_1 m seq m' seq' m'':
+    removal m seq m' ->
+    removal m' seq' m'' ->
+    removal m (seq ++ seq') m''.
+  Proof.
+    intro HRem. induction HRem as [|] ; [done | econstructor ; eauto].
   Qed.
   
-  Inductive removal : Map (list val) -> list (val * val) -> Map (list val) -> Prop :=
+  Lemma removal_app_2 m m' seq seq' :
+    removal m (seq ++ seq') m' ->
+    exists m'', removal m seq m'' /\ removal m'' seq' m'. 
+  Proof.
+    revert m.
+    induction seq as [|[k x] seq IH].
+    - simpl. intros m ?. exists m. split. by constructor 1. assumption.
+    - simpl. intros m Hrem. inversion Hrem as [| ? k' ??????? Hrem']. simplify_eq.
+      specialize (IH (remove_val m k') Hrem'). destruct IH as [m'' [Hseq Hseq']].
+      exists m''. split.
+      by econstructor. assumption.
+  Qed.
+  
+ (* Inductive removal : Map (list val) -> list (val * val) -> Map (list val) -> Prop :=
   | RemovalNil {M M'} : MEquiv M M' -> removal M [] M'
   | RemovalCons {k k' x l M M' M''} :
       as_key k = Some k' ->
@@ -192,15 +257,43 @@ Section model.
       specialize (IH (delete k' M) Hrem'). destruct IH as [M'' [Hseq Hseq']].
       exists M''. split.
       by econstructor. assumption.
+  Qed.*)
+
+  Definition permitted m seq := exists m', removal m seq m'.
+  Definition complete m seq := removal m seq ∅ .
+
+(*  Global Instance permitted_proper : Proper (MEquiv ==> (=) ==> (↔)) permitted.
+  Proof. solve_proper. Qed.*)
+
+  Lemma complete_all_elements m seq:
+    complete m seq ->
+    exists seq', Forall2 (fun '(k, x) '(k', x') => x = x' /\ as_key k' = Some k) seq' seq /\
+                 seq' ≡ₚ all_elements m.
+  Proof.
+    assert (forall (k : Key) (l : list val),
+               Proper (Permutation ==> Permutation) (fun acc => ((fun x => (k, x)) <$> l) ++ acc)).
+    { solve_proper. }
+    assert ( forall A (l1 l2 l3 : list A),
+               l1 ++ l2 ++ l3 ≡ₚ l2 ++ l1 ++ l3).
+    { intros. do 2 rewrite app_assoc. f_equiv. apply Permutation_app_comm. }
+    revert m. induction seq as [|[k x] seq IH].
+    - intros m HCom. exists [].
+      split ; first done. inversion HCom.
+       by rewrite  /all_elements map_fold_empty.
+    - intros m HCom. inversion HCom as [| ??k'?????? Hlookup HRem].
+      specialize (IH _ HRem). destruct IH as [seq' [Hforall HPerm]].
+      exists ((k', x) :: seq'). split.
+      + by apply Forall2_cons.
+      + rewrite HPerm /all_elements /remove_val Hlookup. destruct xs.
+        * rewrite -{2}(insert_id m k' [x]) // -insert_delete.
+          rewrite (map_fold_insert Permutation) //. apply lookup_delete.
+        * rewrite -insert_delete (map_fold_insert Permutation) // ; last apply lookup_delete.
+          rewrite app_comm_cons  -fmap_cons.
+          rewrite -{2}(insert_id m k' (x :: v :: xs)) // -insert_delete.
+          rewrite (map_fold_insert Permutation) //. apply lookup_delete.
   Qed.
-
-  Definition permitted M seq := exists M', removal M seq M'.
-  Definition complete M seq := removal M seq ∅ .
-
-  Global Instance permitted_proper : Proper (MEquiv ==> (=) ==> (↔)) permitted.
-  Proof. solve_proper. Qed.
         
-  Lemma complete_all_elements M seq:
+ (* Lemma complete_all_elements M seq:
     complete M seq ->
     exists seq', Forall2 (fun '(k, x) '(k', x') => x = x' /\ as_key k' = Some k) seq' seq /\
                  seq' ≡ₚ all_elements M.
@@ -241,12 +334,11 @@ Section model.
     
   Global Instance complete_proper : Proper (MEquiv ==> (=) ==> (↔)) complete.
   Proof. solve_proper. Qed.
-
-  
+*)  
       
 End model.
 
-Structure Table Σ Key Hash `{Hashable Σ Key Hash} Map `{FinMap Key Map} : Type :=
+Structure table Σ key hash map `{FinMap key map, heapG Σ, !Hashable Σ key hash} : Type :=
   { table_create : val ;
     table_insert : val ;
     table_lookup : val ;
@@ -254,68 +346,86 @@ Structure Table Σ Key Hash `{Hashable Σ Key Hash} Map `{FinMap Key Map} : Type
     table_cascade : val ;
 
     table_state : Type ;
-    table_in_state : Map (list val) -> table_state -> val -> iProp Σ ;
-    is_cascade : Map (list val) -> val -> list (val * val) -> table_state -> val -> Prop ;
+    table_in_state : map (list val) -> table_state -> val -> iProp Σ ;
+    is_cascade : map (list val) -> val -> list (val * val) -> table_state -> val -> iProp Σ ;
 
-    table_in_state_proper: Proper (MEquiv ==> (=) ==> (=) ==> (⊣⊢)) table_in_state ;
-    is_cascade_proper : Proper (MEquiv ==> (=) ==> (=) ==> (=) ==> (=) ==> (↔)) is_cascade ;
+    table_in_state_wf m state t : (table_in_state m state t → ⌜table_wf m⌝)%I ;
+    is_cascade_persistent m f seq state t : PersistentP (is_cascade m f seq state t) ;
+    
+    (*table_in_state_proper: Proper (MEquiv ==> (=) ==> (=) ==> (⊣⊢)) table_in_state ;
+    is_cascade_proper : Proper (MEquiv ==> (=) ==> (=) ==> (=) ==> (=) ==> (↔)) is_cascade ;*)
     
     table_create_spec (n : nat) : (n > 0)%nat -> WP table_create #n {{t, ∃ state, table_in_state ∅ state t}}%I ;
     
-    table_insert_spec (t k x : val) M state k' :
+    table_insert_spec (t k x : val) m state k' :
       as_key k = Some k' ->
-      {{{table_in_state M state t}}}
+      {{{table_in_state m state t}}}
         table_insert t k x
-        {{{state', RET #(); table_in_state (insert_val M k' x) state' t}}} ;
+        {{{state', RET #(); table_in_state (insert_val m k' x) state' t}}} ;
 
-    table_lookup_spec M state t k k' :
+    table_lookup_spec m state t k k' :
       as_key k = Some k' ->
-      {{{table_in_state M state t}}}
+      {{{table_in_state m state t}}}
         table_lookup t k
-        {{{ RET match head (lookup_all M k') with
-                  Some v => SOMEV v
-                | None => NONEV end ;
-            table_in_state M state t }}} ;
+        {{{ RET match m !! k' with
+                | Some (v :: _) => SOMEV v
+                | _ => NONEV end ;
+            table_in_state m state t }}} ;
 
-    table_fold_spec M state I (f t a : val) :
+ (*   table_fold_spec m state I (f t a : val) :
       (forall k x seq (a' : val),
-          permitted M (seq ++ [(k, x)]) ->
+          permitted m (seq ++ [(k, x)]) ->
           {{I seq a'}} f k x a' {{v,I (seq ++ [(k ,x)]) v }}%I) ->
-      {{{table_in_state M state t ∗ I [] a}}}
+      {{{table_in_state m state t ∗ I [] a}}}
         table_fold f t a
-        {{{v seq, RET v; ⌜complete M seq⌝ ∗ table_in_state M state t ∗ I seq v}}} ;
+        {{{v seq, RET v; ⌜complete m seq⌝ ∗ table_in_state m state t ∗ I seq v}}} ;*)
+    table_fold_spec m state I (f t a : val) :
+      ((∀ k x seq (a' : val),
+           ⌜permitted m (seq ++ [(k,x)])⌝ →
+           {{I seq a'}} f k x a' {{v, I (seq ++ [(k,x)]) v }}) →
+       {{{table_in_state m state t ∗ I [] a}}}
+         table_fold f t a
+       {{{v seq, RET v; ⌜complete m seq⌝ ∗ table_in_state m state t ∗ I seq v}}})%I ;
 
-    is_cascade_spec M f seq state t:
-      is_cascade M f seq state t ->
-      {{{ table_in_state M state t }}}
+   (* is_cascade_spec m f seq state t:
+      is_cascade m f seq state t ->
+      {{{ table_in_state m state t }}}
         f #()
-        {{{v k x f' , RET v; table_in_state M state t ∗
-                             ((⌜v = NONEV⌝ ∗ ⌜complete M seq⌝) ∨
+        {{{v k x f' , RET v; table_in_state m state t ∗
+                             ((⌜v = NONEV⌝ ∗ ⌜complete m seq⌝) ∨
                               (⌜v = SOMEV ((k, x), f')⌝ ∗
-                               ⌜permitted M (seq ++ [(k, x)])⌝ ∗           
-                               ⌜is_cascade M f' (seq ++ [(k, x)]) state t⌝)) }}} ;
+                               ⌜permitted m (seq ++ [(k, x)])⌝ ∗           
+                               ⌜is_cascade m f' (seq ++ [(k, x)]) state t⌝)) }}} ;*)
+    is_cascade_spec m f seq state t:
+      {{{ is_cascade m f seq state t ∗ table_in_state m state t }}}
+        f #()
+      {{{v k x f' , RET v; table_in_state m state t ∗
+                           ((⌜v = NONEV⌝ ∗ ⌜complete m seq⌝) ∨
+                            (⌜v = SOMEV ((k, x), f')⌝ ∗
+                             ⌜permitted m (seq ++ [(k, x)])⌝ ∗           
+                             is_cascade m f' (seq ++ [(k, x)]) state t)) }}};
 
-    table_cascade_spec M state t:
-      {{{table_in_state M state t}}}
+    table_cascade_spec m state t:
+      {{{table_in_state m state t}}}
         table_cascade t
-        {{{f, RET f; ⌜is_cascade M f [] state t⌝ ∗ table_in_state M state t }}}
+        {{{f, RET f; is_cascade m f [] state t ∗ table_in_state m state t }}}
   }.
+Arguments table_create {_ _ _ _ _ _ _ _ _ _ _ _ _ _ _} _.
+Arguments table_insert {_ _ _ _ _ _ _ _ _ _ _ _ _ _ _} _.
+Arguments table_lookup {_ _ _ _ _ _ _ _ _ _ _ _ _ _ _} _.
+Arguments table_fold {_ _ _ _ _ _ _ _ _ _ _ _ _ _ _} _.
+Arguments table_cascade {_ _ _ _ _ _ _ _ _ _ _ _ _ _ _} _.
+Arguments table_state {_ _ _ _ _ _ _ _ _ _ _ _ _ _ _} _.
+Arguments table_in_state {_ _ _ _ _ _ _ _ _ _ _ _ _ _ _} _ _ _ _.
+Arguments is_cascade {_ _ _ _ _ _ _ _ _ _ _ _ _ _ _} _ _ _ _ _ _.
+Arguments table_in_state_wf {_ _ _ _ _ _ _ _ _ _ _ _ _ _ _} _ _ _ _.
+Arguments is_cascade_persistent {_ _ _ _ _ _ _ _ _ _ _ _ _ _ _} _ _ _ _ _ _.
+Arguments table_create_spec {_ _ _ _ _ _ _ _ _ _ _ _ _ _ _} _ _ _.
+Arguments table_insert_spec {_ _ _ _ _ _ _ _ _ _ _ _ _ _ _} _ _ _ _ _ _ _ _ _.
+Arguments table_lookup_spec {_ _ _ _ _ _ _ _ _ _ _ _ _ _ _} _ _ _ _ _ _ _ _.
+Arguments table_fold_spec {_ _ _ _ _ _ _ _ _ _ _ _ _ _ _} _ _ _ _ _ _ _.
+Arguments is_cascade_spec {_ _ _ _ _ _ _ _ _ _ _ _ _ _ _} _ _ _ _ _ _ _.
+Arguments table_cascade_spec {_ _ _ _ _ _ _ _ _ _ _ _ _ _ _} _ _ _ _ _.
 
-Print Implicit table_create.
-
-Arguments table_create {_ _ _ _ _ _ _ _ _ _ _ _ _ _ _ _} _.
-Arguments table_insert {_ _ _ _ _ _ _ _ _ _ _ _ _ _ _ _} _.
-Arguments table_lookup {_ _ _ _ _ _ _ _ _ _ _ _ _ _ _ _} _.
-Arguments table_fold {_ _ _ _ _ _ _ _ _ _ _ _ _ _ _ _} _.
-Arguments table_cascade {_ _ _ _ _ _ _ _ _ _ _ _ _ _ _ _} _.
-Arguments table_state {_ _ _ _ _ _ _ _ _ _ _ _ _ _ _ _} _.
-Arguments table_in_state {_ _ _ _ _ _ _ _ _ _ _ _ _ _ _ _ _} _ _ _.
-Arguments is_cascade {_ _ _ _ _ _ _ _ _ _ _ _ _ _ _ _ _} _ _ _ _ _.
-Arguments table_create_spec {_ _ _ _ _ _ _ _ _ _ _ _ _ _ _ _} _ _ _.
-Arguments table_insert_spec {_ _ _ _ _ _ _ _ _ _ _ _ _ _ _ _ _} _ _ _ _ _ _ _.
-Arguments table_lookup_spec {_ _ _ _ _ _ _ _ _ _ _ _ _ _ _ _ _} _ _ _ _ _ _.
-Arguments table_fold_spec {_ _ _ _ _ _ _ _ _ _ _ _ _ _ _ _ _} _ _ _ _ _ _ _.
-Arguments is_cascade_spec {_ _ _ _ _ _ _ _ _ _ _ _ _ _ _ _ _} _ _ _ _ _ _.
-Arguments table_cascade_spec {_ _ _ _ _ _ _ _ _ _ _ _ _ _ _ _ _} _ _ _.
-
-Existing Instances is_cascade_proper table_in_state_proper.
+Existing Instance is_cascade_persistent.
+(*Existing Instances is_cascade_proper table_in_state_proper.*)
