for_test.v
@@ -4,30 +4,6 @@ From iris.heap_lang Require Import proofmode notation.
 From iris.proofmode Require Import tactics.
 From iris_programs Require Import forloop.
 
-Lemma wp_for `{heapG Σ} P E m n e j `{Closed [j] e}:
-  (m ≤ n)%Z ->
-  forall Φ, 
-  P m -∗
-     □(∀ (i : Z), ⌜m ≤ i < n⌝%Z -∗ P i -∗ ▷ WP (subst' j #i e) @ E {{_, P (1 + i)%Z}}) -∗
-     (∀ v, P n -∗ Φ v ) -∗
-     WP for: j := #m to #n do e @ E {{Φ}}.
-Proof.
-  intros. iIntros "HPm He HΦ".
-  iApply (wp_wand  with "[-HΦ]"). iApply (wp_for with "[] HPm He") ; [done|by wp_value]. eauto.
-Qed.
-
-
-Tactic Notation "wp_for" constr(P) "with" constr(Hs) :=
-  wp_apply (wp_for P with Hs ++ " [] [-]" ) ;
-  [try solve [done | lia | eauto] | ..
-   |let i := fresh in
-    let v := fresh in
-    let Hi := iFresh' "Hi" in
-    let HP := iFresh' "HP" in
-    iIntros "!#" ; iIntros (i) [Hi ; HP] ; iNext ; simpl_subst ; iRevert (i) [Hi; HP] |iIntros (v)].
-
-Tactic Notation "wp_for" constr(P):= wp_for P with "[]".
-
 Lemma for_test2 `{!heapG Σ} l1 l2 (i j : Z) : {{l1 ↦ #i ∗ l2 ↦ #j}} for: "i" := #i to #i + #5 do #l1 <- !#l1 + #1 ;; #42 {{_, l1 ↦ #(i + 5) ∗ l2 ↦ #j }}.
 Proof.
   iIntros "!# [Hl1 Hl2]".
