hashtable_buckets.v
@@ -1,0 +1,313 @@
+From iris_programs.iterators Require Export hashtable_model.
+
+Section buckets.
+  Close Scope Z_scope.
+  Context Σ Key Hash map `{FinMap Key map , heapG Σ, !Hashable Σ Key Hash}.
+
+  Definition bucket_data := list (val * val).
+
+  Fixpoint bucket (kvs : bucket_data) : val :=
+    match kvs with
+    | [] => NONEV
+    | (k, x) :: tl => SOMEV (k, x, bucket tl)
+    end.
+
+  Global Instance bucket_inj : Inj (=) (=) bucket.
+  Proof.
+    intros b1.
+    induction b1 as [|[??]? IH]; intros [|[??]?] Heq; try done.
+    injection Heq. intros ? -> ->. f_equal. by apply IH.
+  Qed.
+  
+  Definition lookup_data `(data : list (list A)) k :=
+    from_option id []
+                (data !! (Hash k mod length data)).
+
+  Definition insert_data `(data : list (list A)) k x :=
+    <[(Hash k mod length data) := x :: lookup_data data k ]> data.
+  
+  Fixpoint bucket_remove k (b : bucket_data) :=
+    match b with
+    | [] => []
+    | (k', x) :: b => if decide (as_key k' = Some k)
+                      then b else (k', x) :: bucket_remove k b
+    end.
+  
+  Definition bucket_filter k (b : bucket_data) :=
+    filter (fun '(k', _) => as_key k' = Some k) b.
+  
+  Lemma bucket_filter_remove k b :
+    tail (bucket_filter k b) = bucket_filter k (bucket_remove k b).
+  Proof.
+    induction b as [|[k' x] b IH].
+    - reflexivity.
+    - unfold bucket_filter, filter. unfold bucket_filter, filter in IH. simpl. case_decide.
+      + done.
+      + simpl. by rewrite decide_False.
+  Qed.
+  
+  Lemma bucket_filter_remove_ne k k' b :
+    k ≠ k' ->
+    bucket_filter k' b = bucket_filter k' (bucket_remove k b).
+  Proof.
+    intro Hne. induction b as [|[k'' x] b IH].
+    - reflexivity.
+    - simpl. case_decide.
+      + unfold bucket_filter, filter, list_filter. rewrite decide_False. done.
+        rewrite (_:as_key k'' = Some k). by injection. assumption. 
+      + simpl. unfold bucket_filter, filter, list_filter. case_decide.
+        * unfold bucket_filter in IH. by rewrite IH.
+        * done.
+  Qed.
+        
+  Lemma lookup_mod `(data : list (list A)) k k' :
+    Hash k mod length data = Hash k' mod length data ->
+    lookup_data data k = lookup_data data k'.
+  Proof.
+    intros Hmod.
+    unfold lookup_data.
+    rewrite Hmod.
+    f_equal.
+  Qed.
+      
+  Lemma lookup_insert_data `(data : list (list A)) k k' x :
+    0 < length data ->
+    Hash k mod length data = Hash k' mod length data ->
+    lookup_data (insert_data data k' x) k = x :: lookup_data data k.
+  Proof.
+    intros Hlen Hmod.
+    unfold insert_data.
+    rewrite (lookup_mod _ _ _ Hmod).
+    rewrite -Hmod.
+    unfold lookup_data at 1.
+    rewrite insert_length.
+    rewrite Hmod.
+    rewrite list_lookup_insert ; [done|].
+    apply mod_bound_pos.
+    apply le_0_n.
+    done.
+  Qed.
+
+  Lemma lookup_insert_data_other `(data : list (list A)) k k' x :
+    0 < length data ->
+    Hash k mod length data ≠ Hash k' mod length data ->
+    lookup_data (insert_data data k' x) k = lookup_data data k.
+  Proof.
+    intros Hlen Hmod.
+    unfold insert_data.
+    unfold lookup_data at 1.
+    rewrite insert_length.
+    rewrite list_lookup_insert_ne ; [|done].
+    by unfold lookup_data.
+  Qed.
+
+  Definition content m (data : list bucket_data) :=
+    map_Forall (fun k l => l = (bucket_filter k (lookup_data data k)).*2) m
+    /\ forall k, m  !! k = None -> [] = bucket_filter k (lookup_data data k).
+      
+  Lemma content_empty n :
+    content ∅ (replicate n []).
+  Proof.
+    split. apply map_Forall_empty.
+    intros. unfold bucket_filter, filter, list_filter, lookup_data.
+    rewrite replicate_length. destruct n.
+    - reflexivity.
+    - rewrite lookup_replicate_2. reflexivity. apply mod_bound_pos ; lia.
+  Qed.
+      
+  Lemma content_insert m data k k' x:
+    0 < length data ->
+    as_key k' = Some k ->
+    content m data ->
+    content (insert_val m k x) (insert_data data k (k', x)).
+  Proof.
+    intros Hlen HKey HContent.
+    split. 
+    - intros k'' l Hlookup.
+      destruct (decide (k = k'')) as [<-|].
+      + rewrite lookup_insert in Hlookup. injection Hlookup as <-.
+        destruct HContent as [Hin Hnin]. specialize (Hin k). specialize (Hnin k).
+        rewrite lookup_insert_data // /bucket_filter /filter /= decide_True //.
+        destruct (m !! k) as [l|]. rewrite (Hin l) //. unfold bucket_filter in Hnin. rewrite -Hnin //.
+      + rewrite lookup_insert_ne in Hlookup ; last assumption.
+        destruct (decide (Hash k mod length data = Hash k'' mod length data)).
+        * rewrite lookup_insert_data ; [| done ..].
+          rewrite /bucket_filter /filter /= decide_False.
+          destruct HContent as [Hin _]. rewrite (Hin _ _ Hlookup) //.
+          rewrite HKey. by injection.
+        * rewrite lookup_insert_data_other //.
+          destruct HContent as [Hin _]. rewrite (Hin _ _ Hlookup) //.
+    - intros k'' Hlookup. destruct HContent as [_ HContent].
+      unfold insert_val in Hlookup. apply lookup_insert_None in Hlookup.
+      destruct (decide (Hash k'' `mod` length data = Hash k `mod` length data)) as [Heq|].
+      + rewrite lookup_insert_data ; [|assumption..].
+        rewrite /bucket_filter /filter /= decide_False. apply HContent. apply Hlookup.
+        destruct Hlookup. rewrite HKey. injection. by intros <-.
+      + rewrite lookup_insert_data_other ; [|assumption..].
+        apply HContent. apply Hlookup.
+  Qed.
+
+  Lemma content_remove m k data:
+    0 < length data ->
+    content m data ->
+    content (remove_val m k)
+            (<[Hash k mod length data
+               := bucket_remove k (lookup_data data k)]>data).
+  Proof.
+    intros Hlen [Hin Hnin].
+    assert (forall k', Hash k' `mod` length data < length data).
+    { intro. apply mod_bound_pos. lia. assumption. }
+    split.
+    - intros k' l. destruct (decide (k = k')) as [<-|].
+      + unfold remove_val. case_eq (m !! k) ; last by intros ->.
+        intros [|?[|]] Hlookup ; [by rewrite lookup_delete..|].
+        rewrite lookup_insert. intro Heq. injection Heq as <-.
+        rewrite {1}/lookup_data insert_length list_lookup_insert // /= -bucket_filter_remove fmap_tail.
+        rewrite -(Hin _ _ Hlookup) //. 
+      + destruct (decide (Hash k `mod` length data = Hash k' `mod` length data)) as [Heq|Hne].
+        * rewrite /lookup_data insert_length Heq list_lookup_insert // /= -bucket_filter_remove_ne //.
+          rewrite lookup_remove_val_ne //. intros Hlookup. rewrite (Hin _ _ Hlookup) //.
+        * rewrite /lookup_data insert_length list_lookup_insert_ne // /=.
+          rewrite lookup_remove_val_ne //. intros Hlookup. rewrite (Hin _ _ Hlookup) //.
+    - intros k' Hlookup. destruct (decide (k = k')) as [<-|].
+      + rewrite {1}/lookup_data insert_length list_lookup_insert /= // -bucket_filter_remove.
+        unfold remove_val in Hlookup. case_eq (m !! k) ; last (intros ; by erewrite <-Hnin).
+        intros [|?[|]] Heq ;[..| rewrite Heq lookup_insert // in Hlookup].
+        all: apply symmetry, (fmap_nil_inv snd), symmetry ;
+          rewrite fmap_tail ; specialize (Hin _ _ Heq) ; rewrite -Hin //.
+      + destruct (decide (Hash k `mod` length data = Hash k' `mod` length data)) as [Heq|Hne].
+        * rewrite /lookup_data insert_length Heq list_lookup_insert // -bucket_filter_remove_ne //.
+          apply Hnin. rewrite lookup_remove_val_ne // in Hlookup .
+        * rewrite /lookup_data insert_length list_lookup_insert_ne //.
+          apply Hnin. rewrite lookup_remove_val_ne // in Hlookup.
+  Qed.
+    
+  Definition have_keys (data : list bucket_data) :=
+    Forall (fun b => Forall (fun '(k, _) => is_Some (as_key k)) b) data.
+  
+  Lemma have_keys_empty n :
+    have_keys (replicate n []).
+  Proof.
+    apply Forall_forall.
+    intros b HbIn.
+    pose proof (elem_of_replicate n [] b) as Hb.
+    setoid_rewrite Hb in HbIn.
+    inversion HbIn as [HbNil _].
+    by rewrite HbNil.
+  Qed.      
+      
+  Lemma have_keys_insert data k k' x:
+    as_key k' = Some k ->
+    have_keys data ->
+    have_keys (insert_data data k (k', x)).
+  Proof.
+    intros HKey Hdata.
+    apply Forall_insert ; [assumption|].
+    apply Forall_cons.
+    split.
+    by exists k.
+    unfold lookup_data.
+    destruct (decide ((Hash k mod length data) < length data)) as [Hlt|Hge].
+    destruct (lookup_lt_is_Some_2 _ _ Hlt) as [b Hb].
+    rewrite Hb. simpl.
+    apply (Forall_lookup_1 _ _ _ _ Hdata Hb).
+    rewrite (lookup_ge_None_2 _ _). by simpl.
+    assert (forall (n m : nat), n <= m <-> ~ m < n) as tmp. intros. lia.
+    by apply tmp.
+  Qed.
+
+  Lemma Forall_keys_remove_bucket k b :
+    Forall (λ '(k, _), is_Some (as_key k)) b ->
+    Forall (λ '(k, _), is_Some (as_key k)) (bucket_remove k b).
+  Proof.
+    induction b as [|[k' x] b IH] .
+    - intro. by apply Forall_nil.
+    - intro Hkeys.
+      pose proof (Forall_cons_1 _ _ _ Hkeys) as [? ?].
+      simpl. case_decide.
+      + assumption.
+      + apply Forall_cons. auto.
+  Qed.
+
+  Lemma have_keys_remove data k:
+    have_keys data ->
+    have_keys (<[Hash k mod length data := bucket_remove k (lookup_data data k)]> data).
+  Proof.
+    intro HKeys.
+    destruct (decide (0 < length data)).
+    - apply Forall_insert. assumption.
+      unfold lookup_data.
+      assert (exists b, data !! (Hash k `mod` length data) = Some b) as [b Hb].
+      { apply lookup_lt_is_Some. apply mod_bound_pos. lia. assumption. }
+      rewrite Hb. simpl.
+      apply Forall_keys_remove_bucket.
+      apply (Forall_lookup_1 _ _ _ _ HKeys Hb).
+    - rewrite (nil_length_inv data).
+      by apply Forall_nil.
+      lia.
+  Qed.
+  
+  Definition no_garbage (data : list bucket_data) :=
+    forall i k,
+      i < length data -> 
+      i ≠ Hash k mod length data ->
+      [] = snd <$> (bucket_filter k
+                                  (from_option
+                                     id []
+                                     (data !! i))).
+
+  Lemma no_garbage_empty n :
+    no_garbage (replicate n []).
+  Proof.
+    intros i k Hi _.
+    rewrite lookup_replicate_2 ; [done|].
+    by rewrite replicate_length in Hi.
+  Qed.
+  
+  Lemma no_garbage_insert data k k' x :
+    as_key k' = Some k ->
+    no_garbage data ->
+    no_garbage (insert_data data k (k', x)).
+  Proof.
+    intros Hkey HNG i k'' Hlen Hi.
+    unfold insert_data in Hi.
+    rewrite insert_length in Hi Hlen.
+    unfold insert_data.
+    destruct (decide (i = Hash k mod length data)).
+    - simplify_eq.
+      rewrite list_lookup_insert ; [|done].
+      simpl. unfold bucket_filter, filter, list_filter.
+      simpl.
+      destruct (decide (k = k'')). 
+      simplify_eq.
+      rewrite decide_False.
+      apply HNG ; [|done]. Nat.order.
+      rewrite Hkey.
+      by injection.
+    - rewrite list_lookup_insert_ne ; [|done].
+      apply HNG ; done.
+  Qed.
+
+  Lemma no_garbage_remove data k:
+    no_garbage data ->
+    no_garbage (<[Hash k mod length data := bucket_remove k (lookup_data data k)]> data).
+  Proof.
+    intros HNG i k' Hlen Hi.
+    rewrite insert_length in Hlen.
+    destruct (decide (i = Hash k `mod` length data)) as [->|].
+    - unfold lookup_data.
+      assert (exists b, data !! (Hash k `mod` length data) = Some b) as [b Hb].
+      { apply lookup_lt_is_Some. apply mod_bound_pos ; lia. }
+      rewrite Hb list_lookup_insert.
+      rewrite -bucket_filter_remove_ne. rewrite -Hb. apply HNG.
+      assumption. by rewrite insert_length in Hi.
+      rewrite insert_length in Hi. intros <-. contradiction.
+      assumption.
+    - rewrite list_lookup_insert_ne. apply HNG.
+      assumption. by rewrite insert_length in Hi. by intros <-.
+  Qed.
+
+End buckets.
+Arguments content _ {_} _ {_ _ _ _ _} _ _.
+Arguments no_garbage _ {_} _ {_ _ _} _.
+Arguments have_keys _ {_ _ _ _} _.
