iterators/modulo.v
@@ -1,0 +1,38 @@
+From iris.proofmode Require Export tactics.
+From iris.heap_lang Require Export lang notation proofmode.
+From iris_programs.iterators Require Import util.
+
+(* A simple implementation of the modulo function. *)
+
+Definition modulo: val :=
+  rec: "mod" "p" :=
+    let: "a" := Fst "p" in
+    let: "b" := Snd "p" in
+    if: "b" = #0 then #0
+    else if: "b" < #0 then -("mod" (-"a", -"b"))
+    else if: "a" < #0 then "mod" ("a" + "b", "b") 
+    else if: "b" ≤ "a" then "mod" ("a" - "b", "b")
+    else "a".
+
+Lemma modulo_spec `{heapG Σ} (m n : Z) :
+  WP modulo (#m, #n) {{v, ⌜v = #(m `mod` n)⌝}}%I.
+Proof.
+  iLöb as "IH" forall (m n).
+  wp_rec. repeat first [wp_proj|wp_lam]. wp_op.
+  - intros Heq. injection Heq as ->. wp_if. by case m.
+  - intros Hne. do 2 apply f_neq in Hne. wp_if. wp_op.
+    + intros _. wp_if. repeat wp_op. wp_bind (modulo _). iApply wp_wand. iApply "IH".
+      iIntros (?) "%". simplify_eq. wp_op. iPureIntro. f_equal.
+      rewrite Zmod_opp_opp Zopp_involutive //.
+    + intros Hn. wp_if. wp_op.
+      * intros Hm. wp_if. wp_op. iApply wp_wand. iApply "IH".
+        iIntros (?) "%". simplify_eq. iPureIntro. f_equal.
+        rewrite -{1}(Zmult_1_l n) Z_mod_plus //. lia.
+      * intros Hm. wp_if. wp_op.
+        -- intros Hle. wp_if. wp_op. iApply wp_wand. iApply "IH".
+           iIntros (?) "%". simplify_eq. iPureIntro.
+           rewrite (_: m - n = m + -1*n); last lia.
+           rewrite Z_mod_plus //. lia.
+        -- intro Hlt. wp_if. iPureIntro. do 2 f_equal. symmetry. apply Zmod_small. lia.
+Qed.
+           
